module Structure.Logic.Constructive.Proofs where

open import Functional as Fn
open import Functional.Instance
open import Logic.Propositional as Logic using (_â†_ ; _â†”_)
open import Logic.Predicate     as Logic hiding (âˆ€â‚—)
import      Lvl
import      Structure.Logic.Constructive.BoundedPredicate
import      Structure.Logic.Constructive.Predicate
import      Structure.Logic.Constructive.Propositional
open import Syntax.Function
open import Type

private variable â„“ â„“â‚— â„“â‚˜â‚— â„“â‚’ â„“â‚š : Lvl.Level
private variable Formula : Type{â„“â‚—}
private variable Proof : Formula â†’ Type{â„“â‚˜â‚—}
private variable Predicate : Type{â„“â‚š}
private variable Domain : Type{â„“â‚’}

module _ (Proof : Formula â†’ Type{â„“â‚˜â‚—}) where
  open Structure.Logic.Constructive.Propositional(Proof)
  private variable X Y Z : Formula

  {-
  module _ â¦ƒ logic : ConstructiveLogic â¦„ where
    [âŸµ][âŸ¶][âˆ§]-[âŸ·]-equivalence : Proof(X âŸ· Y) â†” (Proof(X âŸµ Y) Logic.âˆ§ Proof(X âŸ¶ Y))
    [âŸµ][âŸ¶][âˆ§]-[âŸ·]-equivalence {X} {Y} = Logic.[â†”]-intro
      (p â†¦ âŸ·.intro (âŸµ.elim(Logic.[âˆ§]-elimâ‚— p)) (âŸ¶.elim(Logic.[âˆ§]-elimáµ£ p)))
      (p â†¦ Logic.[âˆ§]-intro (âŸµ.intro (âŸ·.elimâ‚— p)) (âŸ¶.intro (âŸ·.elimáµ£ p)))
  -}

  [âŸ¶]-redundancyâ‚— : â¦ƒ impl : âˆƒ(Implication) â¦„ â†’ Proof(X âŸ¶ (X âŸ¶ Y)) â†’ Proof(X âŸ¶ Y)
  [âŸ¶]-redundancyâ‚— = âŸ¶.intro âˆ˜ swap applyâ‚‚ âˆ˜ (âŸ¶.elim âˆ˜â‚‚ âŸ¶.elim)

  [âŸ·]-reflexivity : âˆ€{_âŸ·_} â†’ â¦ƒ Equivalence(_âŸ·_) â¦„ â†’ Proof(X âŸ· X)
  [âŸ·]-reflexivity = âŸ·.intro id id

  [âŸµ]-to-[âŸ¶] : â¦ƒ con : âˆƒ(Consequence) â¦„ â†’ âˆƒ(Implication)
  âˆƒ.witness [âŸµ]-to-[âŸ¶] = swap(_âŸµ_)
  Implication.intro (âˆƒ.proof [âŸµ]-to-[âŸ¶]) = âŸµ.intro
  Implication.elim  (âˆƒ.proof [âŸµ]-to-[âŸ¶]) = âŸµ.elim

  [âŸ¶]-to-[âŸµ] : â¦ƒ impl : âˆƒ(Implication) â¦„ â†’ âˆƒ(Consequence)
  âˆƒ.witness [âŸ¶]-to-[âŸµ] = swap(_âŸ¶_)
  Consequence.intro (âˆƒ.proof [âŸ¶]-to-[âŸµ]) = âŸ¶.intro
  Consequence.elim  (âˆƒ.proof [âŸ¶]-to-[âŸµ]) = âŸ¶.elim

  [âŸµ][âŸ¶][âˆ§]-to-[âŸ·] : â¦ƒ con : âˆƒ(Consequence) â¦„ â†’ â¦ƒ impl : âˆƒ(Implication) â¦„ â†’ â¦ƒ or : âˆƒ(Conjunction) â¦„ â†’ âˆƒ(Equivalence)
  âˆƒ.witness [âŸµ][âŸ¶][âˆ§]-to-[âŸ·] X Y = (X âŸµ Y) âˆ§ (X âŸ¶ Y)
  Equivalence.intro (âˆƒ.proof [âŸµ][âŸ¶][âˆ§]-to-[âŸ·]) yx xy = âˆ§.intro (âŸµ.intro yx) (âŸ¶.intro xy)
  Equivalence.elimâ‚— (âˆƒ.proof [âŸµ][âŸ¶][âˆ§]-to-[âŸ·])       = âŸµ.elim âˆ˜ âˆ§.elimâ‚—
  Equivalence.elimáµ£ (âˆƒ.proof [âŸµ][âŸ¶][âˆ§]-to-[âŸ·])       = âŸ¶.elim âˆ˜ âˆ§.elimáµ£

  [âŸ¶][âŸ·]-to-[âˆ§] : â¦ƒ impl : âˆƒ(Implication) â¦„ â†’ â¦ƒ eq : âˆƒ(Equivalence) â¦„ â†’ âˆƒ(Conjunction)
  âˆƒ.witness [âŸ¶][âŸ·]-to-[âˆ§] X Y = (X âŸ¶ Y) âŸ· X
  Conjunction.intro (âˆƒ.proof [âŸ¶][âŸ·]-to-[âˆ§]) x y = âŸ·.intro (const(âŸ¶.intro(const y))) (const x)
  Conjunction.elimâ‚— (âˆƒ.proof [âŸ¶][âŸ·]-to-[âˆ§]) xyx = âŸ·.elimáµ£ xyx (âŸ¶.intro(swap applyâ‚‚(âŸ¶.elim âˆ˜ âŸ·.elimâ‚— xyx)))
  Conjunction.elimáµ£ (âˆƒ.proof [âŸ¶][âŸ·]-to-[âˆ§]) xyx = applyâ‚‚(âŸ·.elimáµ£ xyx (âŸ¶.intro(swap applyâ‚‚ (âŸ¶.elim âˆ˜ âŸ·.elimâ‚— xyx)))) (âŸ¶.elim âˆ˜ (âŸ·.elimâ‚— xyx))

  [âˆ¨][âŸ·]-to-[âŸ¶] : â¦ƒ or : âˆƒ(Disjunction) â¦„ â†’ â¦ƒ eq : âˆƒ(Equivalence) â¦„ â†’ âˆƒ(Implication)
  âˆƒ.witness [âˆ¨][âŸ·]-to-[âŸ¶] X Y = (X âˆ¨ Y) âŸ· Y
  Implication.intro (âˆƒ.proof [âˆ¨][âŸ·]-to-[âŸ¶])       = âŸ·.intro âˆ¨.introáµ£ âˆ˜ swap âˆ¨.elim id
  Implication.elim  (âˆƒ.proof [âˆ¨][âŸ·]-to-[âŸ¶]) xyy x = âŸ·.elimáµ£ xyy (âˆ¨.introâ‚— x)

  [âˆ§][âŸ·]-to-[âŸ¶] : â¦ƒ and : âˆƒ(Conjunction) â¦„ â†’ â¦ƒ eq : âˆƒ(Equivalence) â¦„ â†’ âˆƒ(Implication)
  âˆƒ.witness [âˆ§][âŸ·]-to-[âŸ¶] X Y = (X âˆ§ Y) âŸ· X
  Implication.intro (âˆƒ.proof [âˆ§][âŸ·]-to-[âŸ¶]) xy    = âŸ·.intro (x â†¦ âˆ§.intro x (xy x)) âˆ§.elimâ‚—
  Implication.elim  (âˆƒ.proof [âˆ§][âŸ·]-to-[âŸ¶]) xyx x = âˆ§.elimáµ£(âŸ·.elimâ‚— xyx x)

  [Â¬][âŠ¤]-to-[âŠ¥] : â¦ƒ neg : âˆƒ(Negation) â¦„ â†’ â¦ƒ top : âˆƒ(Top) â¦„ â†’ âˆƒ(Bottom)
  âˆƒ.witness [Â¬][âŠ¤]-to-[âŠ¥] = Â¬ âŠ¤
  Bottom.elim (âˆƒ.proof [Â¬][âŠ¤]-to-[âŠ¥]) = Â¬.elim âŠ¤.intro

  [Â¬][âŠ¥]-to-[âŠ¤] : â¦ƒ neg : âˆƒ(Negation) â¦„ â†’ â¦ƒ bot : âˆƒ(Bottom) â¦„ â†’ âˆƒ(Top)
  âˆƒ.witness [Â¬][âŠ¥]-to-[âŠ¤] = Â¬ âŠ¥
  Top.intro (âˆƒ.proof [Â¬][âŠ¥]-to-[âŠ¤]) = Â¬.intro{Y = âŠ¥} âŠ¥.elim âŠ¥.elim

  {- TODO: Move these to Classical
  [Â¬][âˆ¨]-to-[âˆ§] : â¦ƒ neg : âˆƒ(Negation) â¦„ â†’ â¦ƒ or : âˆƒ(Disjunction) â¦„ â†’ âˆƒ(Conjunction)
  âˆƒ.witness [Â¬][âˆ¨]-to-[âˆ§] X Y = Â¬((Â¬ X) âˆ¨ (Â¬ Y))
  Conjunction.intro (âˆƒ.proof [Â¬][âˆ¨]-to-[âˆ§]) {X} x y = Â¬.intro{Y = X} (âˆ¨.elim (Â¬.elim x) (Â¬.elim y)) (âˆ¨.elim (Â¬.elim x) (Â¬.elim y))
  Conjunction.elimâ‚— (âˆƒ.proof [Â¬][âˆ¨]-to-[âˆ§]) nnxny = Â¬.elim (âˆ¨.introâ‚— (Â¬.intro {!!} {!!})) nnxny
  Conjunction.elimáµ£ (âˆƒ.proof [Â¬][âˆ¨]-to-[âˆ§]) nnxny = {!!}

  [Â¬][âˆ§]-to-[âˆ¨] : â¦ƒ neg : âˆƒ(Negation) â¦„ â†’ â¦ƒ and : âˆƒ(Conjunction) â¦„ â†’ âˆƒ(Disjunction)
  âˆƒ.witness [Â¬][âˆ§]-to-[âˆ¨] X Y = Â¬((Â¬ X) âˆ§ (Â¬ Y))
  Disjunction.introâ‚— (âˆƒ.proof [Â¬][âˆ§]-to-[âˆ¨]) {X} x = Â¬.intro {Y = X} (Â¬.elim x âˆ˜ âˆ§.elimâ‚—) (Â¬.elim x âˆ˜ âˆ§.elimâ‚—)
  Disjunction.introáµ£ (âˆƒ.proof [Â¬][âˆ§]-to-[âˆ¨]) {X} y = Â¬.intro {Y = X} (Â¬.elim y âˆ˜ âˆ§.elimáµ£) (Â¬.elim y âˆ˜ âˆ§.elimáµ£)
  Disjunction.elim   (âˆƒ.proof [Â¬][âˆ§]-to-[âˆ¨]) xz yz nnxny = {!!}
  -- Â¬.elim {!!} nnxny
  -}

  [âŸ·]-to-[âŠ¤] : Formula â†’ â¦ƒ eq : âˆƒ(Equivalence) â¦„ â†’ âˆƒ(Top)
  âˆƒ.witness ([âŸ·]-to-[âŠ¤] Ï†) = Ï† âŸ· Ï†
  Top.intro (âˆƒ.proof ([âŸ·]-to-[âŠ¤] Ï†)) = [âŸ·]-reflexivity

  [âŸ·][âŠ¥]-to-[Â¬] : â¦ƒ eq : âˆƒ(Equivalence) â¦„ â†’ â¦ƒ bot : âˆƒ(Bottom) â¦„ â†’ âˆƒ(Negation)
  âˆƒ.witness [âŸ·][âŠ¥]-to-[Â¬] = _âŸ· âŠ¥
  Negation.intro (âˆƒ.proof [âŸ·][âŠ¥]-to-[Â¬]) xy xyâŠ¥ = âŸ·.intro âŠ¥.elim ((âŸ·.elimáµ£ âˆ˜ xyâŠ¥) âˆ˜â‚› xy)
  Negation.elim  (âˆƒ.proof [âŸ·][âŠ¥]-to-[Â¬])        = âŠ¥.elim âˆ˜â‚‚ swap âŸ·.elimáµ£

  [âŸ¶][âŠ¥]-to-[Â¬] : â¦ƒ eq : âˆƒ(Implication) â¦„ â†’ â¦ƒ bot : âˆƒ(Bottom) â¦„ â†’ âˆƒ(Negation)
  âˆƒ.witness [âŸ¶][âŠ¥]-to-[Â¬] = _âŸ¶ âŠ¥
  Negation.intro (âˆƒ.proof [âŸ¶][âŠ¥]-to-[Â¬]) xy xyâŠ¥ = âŸ¶.intro ((swap âŸ¶.elim âˆ˜ xy) âˆ˜â‚› xyâŠ¥)
  Negation.elim  (âˆƒ.proof [âŸ¶][âŠ¥]-to-[Â¬])        = âŠ¥.elim âˆ˜â‚‚ swap âŸ¶.elim

  [âˆ¨][âŸ·][âŠ¥]-adequacy : â¦ƒ or : âˆƒ(Disjunction) â¦„ â†’ â¦ƒ eq : âˆƒ(Equivalence) â¦„ â†’ â¦ƒ bot : âˆƒ(Bottom) â¦„ â†’ Logic
  Logic.top         [âˆ¨][âŸ·][âŠ¥]-adequacy = [âŸ·]-to-[âŠ¤] âŠ¥
  Logic.implication [âˆ¨][âŸ·][âŠ¥]-adequacy = [âˆ¨][âŸ·]-to-[âŸ¶]
  Logic.negation    [âˆ¨][âŸ·][âŠ¥]-adequacy = [âŸ·][âŠ¥]-to-[Â¬]
  Logic.conjunction [âˆ¨][âŸ·][âŠ¥]-adequacy = [âŸ¶][âŸ·]-to-[âˆ§] where instance _ = Logic.implication [âˆ¨][âŸ·][âŠ¥]-adequacy
  Logic.consequence [âˆ¨][âŸ·][âŠ¥]-adequacy = [âŸ¶]-to-[âŸµ]    where instance _ = Logic.implication [âˆ¨][âŸ·][âŠ¥]-adequacy

  [âŸ¶][âˆ§][âˆ¨][âŠ¤][âŠ¥]-adequacy : â¦ƒ impl : âˆƒ(Implication) â¦„ â†’ â¦ƒ and : âˆƒ(Conjunction) â¦„ â†’ â¦ƒ or : âˆƒ(Disjunction) â¦„ â†’ â¦ƒ top : âˆƒ(Top) â¦„ â†’ â¦ƒ bot : âˆƒ(Bottom) â¦„ â†’ Logic
  Logic.consequence [âŸ¶][âˆ§][âˆ¨][âŠ¤][âŠ¥]-adequacy = [âŸ¶]-to-[âŸµ]
  Logic.equivalence [âŸ¶][âˆ§][âˆ¨][âŠ¤][âŠ¥]-adequacy = [âŸµ][âŸ¶][âˆ§]-to-[âŸ·] where instance _ = Logic.consequence [âŸ¶][âˆ§][âˆ¨][âŠ¤][âŠ¥]-adequacy
  Logic.negation    [âŸ¶][âˆ§][âˆ¨][âŠ¤][âŠ¥]-adequacy = [âŸ¶][âŠ¥]-to-[Â¬]

module _ (Proof : Formula â†’ Type{â„“â‚˜â‚—}) where
  open Structure.Logic.Constructive.Propositional(Proof)
  private variable X Y Z : Formula

  open import Data.Tuple as Tuple using ()

  [âŠ¤]-preserving-type : â¦ƒ top : âˆƒ(Top) â¦„ â†’ Proof(âŠ¤) â†” Logic.âŠ¤
  Tuple.left  [âŠ¤]-preserving-type = const âŠ¤.intro
  Tuple.right [âŠ¤]-preserving-type = const Logic.[âŠ¤]-intro

  [âˆ§]-preserving-type : â¦ƒ and : âˆƒ(Conjunction) â¦„ â†’ Proof(X âˆ§ Y) â†” (Proof(X) Logic.âˆ§ Proof(Y))
  Tuple.left  [âˆ§]-preserving-type (Logic.[âˆ§]-intro x y) = âˆ§.intro x y
  Tuple.right [âˆ§]-preserving-type xy                    = Logic.[âˆ§]-intro (âˆ§.elimâ‚— xy) (âˆ§.elimáµ£ xy)

  [âˆ¨]-preserving-type : â¦ƒ or : âˆƒ(Disjunction) â¦„ â†’ Proof(X âˆ¨ Y) â† (Proof(X) Logic.âˆ¨ Proof(Y))
  [âˆ¨]-preserving-type = Logic.[âˆ¨]-elim âˆ¨.introâ‚— âˆ¨.introáµ£

  [âŸ¶]-preserving-type : â¦ƒ impl : âˆƒ(Implication) â¦„ â†’ Proof(X âŸ¶ Y) â†” (Proof(X) â†’ Proof(Y))
  Tuple.left  [âŸ¶]-preserving-type = âŸ¶.intro
  Tuple.right [âŸ¶]-preserving-type = âŸ¶.elim

  [âŸµ]-preserving-type : â¦ƒ cons : âˆƒ(Consequence) â¦„ â†’ Proof(X âŸµ Y) â†” (Proof(X) â† Proof(Y))
  Tuple.left  [âŸµ]-preserving-type = âŸµ.intro
  Tuple.right [âŸµ]-preserving-type = âŸµ.elim

  [âŸ·]-preserving-type : â¦ƒ eq : âˆƒ(Equivalence) â¦„ â†’ Proof(X âŸ· Y) â†” (Proof(X) â†” Proof(Y))
  Tuple.left  [âŸ·]-preserving-type xy = âŸ·.intro (Logic.[â†”]-to-[â†] xy) (Logic.[â†”]-to-[â†’] xy)
  Tuple.right [âŸ·]-preserving-type xy = Logic.[â†”]-intro (âŸ·.elimâ‚— xy) (âŸ·.elimáµ£ xy)

  {-
  module Test â¦ƒ logic : Logic â¦„ where
    pure : âˆ€{A : Formula} â†’ Proof(A) â†’ Proof(A)
    pure = id

    _<*>_ : âˆ€{A B : Formula} â†’ Proof(A âŸ¶ B) â†’ Proof(A) â†’ Proof(B)
    _<*>_ = âŸ¶.elim

    test : âˆ€{A B} â†’ Proof(A âŸ¶ (A âŸ¶ B)) â†’ Proof(A) â†’ Proof(B)
    test ab a = â¦‡ ab a a â¦ˆ

  module Test2 â¦ƒ logic : ConstructiveLogic â¦„ {Obj : Type{â„“}} where
    private variable P : Obj â†’ Formula

    module _ â¦ƒ all : âˆƒ(Universal) â¦„ where
      pure : âˆ€{A : Formula} â†’ Proof(A) â†’ Proof(A)
      pure = id

      _<*>_ : âˆ€{P : Obj â†’ Formula} â†’ Proof(âˆ€â‚— P) â†’ (x : Obj) â†’ Proof(P(x))
      _<*>_ = âˆ€â‚—.elim

      test : âˆ€{A : Obj â†’ Obj â†’ Formula} â†’ Proof(âˆ€â‚—(x â†¦ âˆ€â‚—(y â†¦ A x y))) â†’ (x : Obj) â†’ Proof(A x x)
      test a x  = â¦‡ a x x â¦ˆ
  -}

module _ where
  open import Data
  open import Data.Tuple
  open import Data.Either as Either
  open        Structure.Logic.Constructive.BoundedPredicate renaming (Logic to BoundedPredicateLogic)
  open        Structure.Logic.Constructive.Predicate        renaming (Logic to PredicateLogic)
  open        Structure.Logic.Constructive.Propositional    renaming (Logic to PropositionalLogic)

  instance
    typePropositionalLogic : PropositionalLogic{Formula = Type{â„“}} id
    PropositionalLogic.bottom      typePropositionalLogic = [âˆƒ]-intro Empty     â¦ƒ record{elim = empty} â¦„
    PropositionalLogic.top         typePropositionalLogic = [âˆƒ]-intro Unit      â¦ƒ record{intro = <>} â¦„
    PropositionalLogic.implication typePropositionalLogic = [âˆƒ]-intro _â†’á¶ _      â¦ƒ record{intro = _$_ ; elim = id} â¦„
    PropositionalLogic.conjunction typePropositionalLogic = [âˆƒ]-intro _â¨¯_       â¦ƒ record{intro = _,_ ; elimâ‚— = left ; elimáµ£ = right} â¦„
    PropositionalLogic.disjunction typePropositionalLogic = [âˆƒ]-intro _â€–_       â¦ƒ record{introâ‚— = Left ; introáµ£ = Right ; elim = Either.map1} â¦„
    PropositionalLogic.consequence typePropositionalLogic = [âˆƒ]-intro _â†á¶ _      â¦ƒ record{intro = id ; elim = _$_} â¦„
    PropositionalLogic.equivalence typePropositionalLogic = [âˆƒ]-intro Logic._â†”_ â¦ƒ record{intro = _,_ ; elimâ‚— = left ; elimáµ£ = right} â¦„
    PropositionalLogic.negation    typePropositionalLogic = [âˆƒ]-intro Logic.Â¬_  â¦ƒ record{intro = Fn.swap(_âˆ˜â‚›_) ; elim = empty âˆ˜â‚‚ apply} â¦„

  instance
    typePredicateLogic : âˆ€{T : Type{â„“â‚’}} â†’ PredicateLogic{Formula = Type{â„“â‚’ Lvl.âŠ” â„“â‚—}} id {Predicate = T â†’ Type{â„“â‚’ Lvl.âŠ” â„“â‚—}} {Domain = T} id
    PredicateLogic.universal   typePredicateLogic = [âˆƒ]-intro Logic.âˆ€â‚— â¦ƒ record{intro = id ; elim = id} â¦„
    PredicateLogic.existential typePredicateLogic = [âˆƒ]-intro Logic.âˆƒ  â¦ƒ record{intro = \{_}{x} p â†’ Logic.[âˆƒ]-intro x â¦ƒ p â¦„ ; elim = Logic.[âˆƒ]-elim} â¦„

  open import Type.Dependent.Sigma
  
  instance
    typeBoundedPredicateLogic : âˆ€{T : Type{â„“â‚’}} â†’ BoundedPredicateLogic{Formula = Type{â„“â‚’ Lvl.âŠ” â„“â‚—}} id {Predicate = (x : T) â†’ âˆ€{B : T â†’ Type{â„“â‚’ Lvl.âŠ” â„“â‚—}} â†’ B(x) â†’ Type{â„“â‚’ Lvl.âŠ” â„“â‚—}} {Domain = T} id
    BoundedPredicateLogic.universal   typeBoundedPredicateLogic = [âˆƒ]-intro (\B P â†’ âˆ€{x} â†’ (bx : B(x)) â†’ P(x){B}(bx)) â¦ƒ record{intro = \p bx â†’ p bx ; elim = \p bx â†’ p bx} â¦„
    BoundedPredicateLogic.existential typeBoundedPredicateLogic = [âˆƒ]-intro (\B P â†’ Logic.âˆƒ(x â†¦ Î£(B(x)) (P(x){B}))) â¦ƒ record{intro = \{_}{x} bx p â†’ Logic.[âˆƒ]-intro x â¦ƒ intro bx p â¦„ ; elim = \p â†’ Logic.[âˆƒ]-elim (\(intro bx px) â†’ p bx px)} â¦„

  {- TODO: Maybe have some more assumptions
  boundedPredicateLogic-to-predicateLogic : âˆ€{Formula Domain Predicate : Type{â„“â‚’}}{Proof : Formula â†’ Type}{_$_} â†’ BoundedPredicateLogic{Formula = Formula} Proof {Predicate = Predicate} {Domain = Domain} (_$_) â†’ PredicateLogic{Formula = Formula} Proof {Predicate = (Domain â†’ Formula) â¨¯ Predicate} {Domain = Î£(Predicate â¨¯ Domain) (\(P , x) â†’ Proof((P $ x) {{!!}} {!!}))} {!!}
  PredicateLogic.propositional (boundedPredicateLogic-to-predicateLogic L) = BoundedPredicateLogic.propositional L
  âˆƒ.witness (PredicateLogic.universal (boundedPredicateLogic-to-predicateLogic L)) (B , P) = âˆƒ.witness (BoundedPredicateLogic.universal L) B P
  Universal.intro (âˆƒ.proof (PredicateLogic.universal (boundedPredicateLogic-to-predicateLogic L))) {B , P} p = BoundedUniversal.intro
                                                                                                         (âˆƒ.proof (BoundedPredicateLogic.universal L)) (\{x} pp â†’ p{intro (P , x) {!!}})
  Universal.elim (âˆƒ.proof (PredicateLogic.universal (boundedPredicateLogic-to-predicateLogic L))) = {!!}
  âˆƒ.witness (PredicateLogic.existential (boundedPredicateLogic-to-predicateLogic L)) (B , P) = âˆƒ.witness (BoundedPredicateLogic.existential L) B P
  Existential.intro (âˆƒ.proof (PredicateLogic.existential (boundedPredicateLogic-to-predicateLogic L))) = {!!}
  Existential.elim (âˆƒ.proof (PredicateLogic.existential (boundedPredicateLogic-to-predicateLogic L))) = {!!}
  -}

  {- TODO: Seems to need a duplicate (Domain â†’ Formula) in Predicate. Also, does not work with this generality
  boundedPredicateLogic-to-predicateLogic : âˆ€{_$_} â†’ BoundedPredicateLogic{Formula = Formula} Proof {Predicate = Predicate} {Domain = Domain} (_$_) â†’ PredicateLogic{Formula = Formula} Proof {Predicate = Predicate} {Domain = Î£((Domain â†’ Formula) â¨¯ Domain) (\(B , x) â†’ Proof(B(x)))} (\P (intro(B , x) bx) â†’ (P $ x) {B} bx)
  PredicateLogic.propositional (boundedPredicateLogic-to-predicateLogic L) = BoundedPredicateLogic.propositional L
  PredicateLogic.universal (boundedPredicateLogic-to-predicateLogic L) = [âˆƒ]-intro {!!} â¦ƒ record{intro = {!!} ; elim = {!!}} â¦„
  PredicateLogic.existential (boundedPredicateLogic-to-predicateLogic L) = [âˆƒ]-intro {!!} â¦ƒ record{intro = {!!} ; elim = {!!}} â¦„
  -}

  {-instance
    typeBoundedPredicateLogic : âˆ€{T : Type{â„“â‚’}}{B : T â†’ Type{â„“}} â†’ PredicateLogic{Formula = Type{â„“â‚’ Lvl.âŠ” â„“â‚— Lvl.âŠ” â„“}} id {Predicate = (x : T) â†’ â¦ƒ B(x) â¦„ â†’ Type{â„“â‚’ Lvl.âŠ” â„“â‚— Lvl.âŠ” â„“}} {Domain = Î£ T B} (\f (intro x b) â†’ f x â¦ƒ b â¦„)
    PredicateLogic.universal   (typeBoundedPredicateLogic {B = B}) = [âˆƒ]-intro (f â†¦ (âˆ€{x} â¦ƒ bx â¦„ â†’ f(x) â¦ƒ bx â¦„)) â¦ƒ record{intro = \px â†’ px ; elim = \{P} px {x} â†’ px{Î£.left x} â¦ƒ Î£.right x â¦„} â¦„
    PredicateLogic.existential (typeBoundedPredicateLogic {B = B}) = [âˆƒ]-intro (f â†¦ Logic.âˆƒ(x â†¦ Î£(B(x)) (bx â†¦ f x â¦ƒ bx â¦„)) ) â¦ƒ record{intro = {!!} ; elim = {!!}} â¦„
  -}

  import      Logic.Classical.DoubleNegated as DoubleNegated
  open import Logic.Names
  import      Logic.Propositional.Theorems as Logic
  instance
    doubleNegatedTypeLogic : PropositionalLogic{â„“â‚˜â‚— = Lvl.ğŸ}(Logic.Â¬Â¬_)
    PropositionalLogic.bottom      doubleNegatedTypeLogic = Logic.[âˆƒ]-intro Logic.âŠ¥     â¦ƒ record{elim = DoubleNegated.[âŠ¥]-elim} â¦„
    PropositionalLogic.top         doubleNegatedTypeLogic = Logic.[âˆƒ]-intro Logic.âŠ¤     â¦ƒ record{intro = DoubleNegated.[âŠ¤]-intro} â¦„
    PropositionalLogic.implication doubleNegatedTypeLogic = Logic.[âˆƒ]-intro (_â†’á¶ _)      â¦ƒ record{intro = DoubleNegated.[â†’]-intro ; elim = DoubleNegated.[â†’]-elim} â¦„
    PropositionalLogic.conjunction doubleNegatedTypeLogic = Logic.[âˆƒ]-intro (Logic._âˆ§_) â¦ƒ record{intro = DoubleNegated.[âˆ§]-intro ; elimâ‚— = DoubleNegated.[âˆ§]-elimâ‚— ; elimáµ£ = DoubleNegated.[âˆ§]-elimáµ£} â¦„
    PropositionalLogic.disjunction doubleNegatedTypeLogic = Logic.[âˆƒ]-intro (Logic._âˆ¨_) â¦ƒ record{introâ‚— = DoubleNegated.[âˆ¨]-introâ‚— ; introáµ£ = DoubleNegated.[âˆ¨]-introáµ£ ; elim = DoubleNegated.[âˆ¨]-elim} â¦„
    PropositionalLogic.consequence doubleNegatedTypeLogic = Logic.[âˆƒ]-intro (Logic._â†_) â¦ƒ record{intro = DoubleNegated.[â†]-intro ; elim = DoubleNegated.[â†’]-elim} â¦„
    PropositionalLogic.equivalence doubleNegatedTypeLogic = Logic.[âˆƒ]-intro (Logic._â†”_) â¦ƒ record{intro = DoubleNegated.[â†”]-intro ; elimâ‚— = DoubleNegated.[â†”]-elimâ‚— ; elimáµ£ = DoubleNegated.[â†”]-elimáµ£} â¦„
    PropositionalLogic.negation    doubleNegatedTypeLogic = Logic.[âˆƒ]-intro (Logic.Â¬_)  â¦ƒ record{intro = Fn.swap(_âˆ˜â‚›_) ; elim = const âˆ˜â‚‚ apply} â¦„

  open import Data.Boolean
  import      Data.Boolean.Operators
  open        Data.Boolean.Operators.Programming
  open import Data.Boolean.Stmt
  open import Data.Boolean.Stmt.Logic
  instance
    booleanLogic : PropositionalLogic IsTrue
    PropositionalLogic.bottom      booleanLogic = [âˆƒ]-intro ğ¹    â¦ƒ record{elim = Logic.[âŠ¥]-elim âˆ˜ IsTrue.[ğ¹]-elim} â¦„
    PropositionalLogic.top         booleanLogic = [âˆƒ]-intro ğ‘‡    â¦ƒ record{intro = IsTrue.[ğ‘‡]-intro} â¦„
    PropositionalLogic.conjunction booleanLogic = [âˆƒ]-intro _&&_ â¦ƒ record{intro = IsTrue.[âˆ§]-intro ; elimâ‚— = IsTrue.[âˆ§]-elimâ‚— ; elimáµ£ = IsTrue.[âˆ§]-elimáµ£} â¦„
    PropositionalLogic.disjunction booleanLogic = [âˆƒ]-intro _||_ â¦ƒ record{introâ‚— = IsTrue.[âˆ¨]-introâ‚— ; introáµ£ = IsTrue.[âˆ¨]-introáµ£ ; elim = IsTrue.[âˆ¨]-elim} â¦„
    PropositionalLogic.negation    booleanLogic = [âˆƒ]-intro !    â¦ƒ record{intro = IsTrue.[!]-intro ; elim = IsTrue.[!]-elim} â¦„
    PropositionalLogic.implication booleanLogic = [âˆƒ]-intro _â†’?_ â¦ƒ record{intro = IsTrue.[â†’?]-intro ; elim = IsTrue.[â†’?]-elim} â¦„
    PropositionalLogic.consequence booleanLogic = [âˆƒ]-intro _â†?_ â¦ƒ record{intro = IsTrue.[â†?]-intro ; elim = IsTrue.[â†?]-elim} â¦„
    PropositionalLogic.equivalence booleanLogic = [âˆƒ]-intro _==_ â¦ƒ record{intro = IsTrue.[==]-intro ; elimâ‚— = IsTrue.[==]-elimâ‚— ; elimáµ£ = IsTrue.[==]-elimáµ£} â¦„

  booleanPredicateLogic : âˆ€{T : Type{â„“}}{all exist : (T â†’ Bool) â†’ Bool} â†’ (âˆ€{P} â†’ (âˆ€{x} â†’ IsTrue(P(x))) â†” IsTrue(all P)) â†’ (âˆ€{P} â†’ (Logic.âˆƒ(x â†¦ IsTrue(P(x)))) â†” IsTrue(exist P)) â†’ PredicateLogic IsTrue {Domain = T} id
  PredicateLogic.universal   (booleanPredicateLogic {all = all} {exist = exist} all-eq exist-eq) = [âˆƒ]-intro all   â¦ƒ record{intro = Logic.[â†”]-to-[â†’] all-eq ; elim = Logic.[â†”]-to-[â†] all-eq} â¦„
  PredicateLogic.existential (booleanPredicateLogic {all = all} {exist = exist} all-eq exist-eq) = [âˆƒ]-intro exist â¦ƒ record{intro = Logic.[â†”]-to-[â†’] exist-eq âˆ˜ (p â†¦ [âˆƒ]-intro _ â¦ƒ p â¦„) ; elim = p â†¦ ep â†¦ p(Logic.[âˆƒ]-proof(Logic.[â†”]-to-[â†] exist-eq ep))} â¦„
