open import Formalization.PredicateLogic.Signature

module Formalization.PredicateLogic.Classical.Semantics.Homomorphism (ğ” : Signature) where
open Signature(ğ”)

import      Lvl
open import Data
open import Data.Boolean
open import Data.Boolean.Stmt
open import Data.ListSized
open import Data.ListSized.Functions
open import Formalization.PredicateLogic.Classical.Semantics(ğ”)
open import Formalization.PredicateLogic.Syntax(ğ”)
open import Functional using (_âˆ˜_ ; _âˆ˜â‚‚_ ; _â†_)
open import Logic.Propositional as Logic using (_â†”_)
import      Logic.Predicate     as Logic
open import Numeral.Finite
open import Numeral.Finite.Bound
open import Numeral.Natural
open import Relator.Equals
open import Relator.Equals.Proofs.Equiv
open import Sets.PredicateSet using (PredSet)
open        Sets.PredicateSet.BoundedQuantifiers
open import Structure.Function.Domain
open import Syntax.Function
open import Type.Dependent.Sigma renaming (intro to _,_)
open import Type.Properties.Decidable
open import Type

private variable â„“ â„“â‚˜ â„“â‚˜â‚ â„“â‚˜â‚‚ â„“â‚‘ : Lvl.Level
private variable P : Type{â„“â‚š}
private variable args n vars : â„•
private variable ğ” : Model

private variable A B C S : Model{â„“â‚˜}
private variable fi : Obj n
private variable ri : Prop n
private variable xs : List(dom(S))(n)

record Homomorphism (A : Model{â„“â‚˜â‚}) (B : Model{â„“â‚˜â‚‚}) (f : dom(A) â†’ dom(B)) : Type{â„“â‚š Lvl.âŠ” â„“â‚’ Lvl.âŠ” Lvl.of(Type.of A) Lvl.âŠ” Lvl.of(Type.of B)} where
  field
    preserve-functions : âˆ€{xs} â†’ (f(fn(A) fi xs) â‰¡ fn(B) fi (map f xs))
    preserve-relations : âˆ€{xs} â†’ IsTrue(rel(A) ri xs) â†’ IsTrue(rel(B) ri (map f xs))

_â†’â‚›â‚œáµ£áµ¤_ : Model{â„“â‚˜â‚} â†’ Model{â„“â‚˜â‚‚} â†’ Type
A â†’â‚›â‚œáµ£áµ¤ B = Logic.âˆƒ(Homomorphism A B)

record Embedding (A : Model{â„“â‚˜â‚}) (B : Model{â„“â‚˜â‚‚}) (f : dom(A) â†’ dom(B)) : Type{â„“â‚š Lvl.âŠ” â„“â‚’ Lvl.âŠ” Lvl.of(Type.of A) Lvl.âŠ” Lvl.of(Type.of B)} where
  constructor intro
  field
    â¦ƒ homomorphism â¦„ : Homomorphism(A)(B)(f)
    â¦ƒ injection â¦„    : Injective(f)
    preserve-relations-converse : âˆ€{xs} â†’ IsTrue(rel(A) ri xs) â† IsTrue(rel(B) ri (map f xs))

open import Data
open import Data.Boolean.Stmt
open import Data.ListSized.Proofs
open import Functional
open import Function.Equals
open import Function.Proofs
open import Functional.Instance
open import Logic.Predicate
open import Structure.Function
open import Structure.Operator
open import Structure.Relator.Properties
open import Structure.Relator
open import Syntax.Transitivity

idâ‚›â‚œáµ£áµ¤ : A â†’â‚›â‚œáµ£áµ¤ A
âˆƒ.witness idâ‚›â‚œáµ£áµ¤ = id
Homomorphism.preserve-functions (âˆƒ.proof (idâ‚›â‚œáµ£áµ¤ {A = A})) {n} {fi} {xs} = congruenceâ‚(fn A fi) (symmetry(_â‰¡_) (_âŠœ_.proof map-id))
Homomorphism.preserve-relations (âˆƒ.proof (idâ‚›â‚œáµ£áµ¤ {A = A})) {n} {ri} {xs} = substituteâ‚â‚—(IsTrue âˆ˜ rel A ri) (_âŠœ_.proof map-id)

_âˆ˜â‚›â‚œáµ£áµ¤_ : let _ = A ; _ = B ; _ = C in (B â†’â‚›â‚œáµ£áµ¤ C) â†’ (A â†’â‚›â‚œáµ£áµ¤ B) â†’ (A â†’â‚›â‚œáµ£áµ¤ C)
âˆƒ.witness (([âˆƒ]-intro f) âˆ˜â‚›â‚œáµ£áµ¤ ([âˆƒ]-intro g)) = f âˆ˜ g
Homomorphism.preserve-functions (âˆƒ.proof (_âˆ˜â‚›â‚œáµ£áµ¤_ {A = A} {B = B} {C = C} ([âˆƒ]-intro f â¦ƒ hom-f â¦„) ([âˆƒ]-intro g â¦ƒ hom-g â¦„))) {fi = fi} {xs} =
  congruenceâ‚(f) (Homomorphism.preserve-functions hom-g)
  ğŸ– Homomorphism.preserve-functions hom-f
  ğŸ– congruenceâ‚(fn C fi) (symmetry(_â‰¡_) (_âŠœ_.proof (map-[âˆ˜] {f = f}{g = g}) {xs}))
Homomorphism.preserve-relations (âˆƒ.proof (_âˆ˜â‚›â‚œáµ£áµ¤_ {A = A} {B = B} {C = C} ([âˆƒ]-intro f â¦ƒ hom-f â¦„) ([âˆƒ]-intro g â¦ƒ hom-g â¦„))) {ri = ri} {xs} =
  substituteâ‚â‚—(IsTrue âˆ˜ rel C ri) (_âŠœ_.proof map-[âˆ˜] {xs})
  âˆ˜ Homomorphism.preserve-relations hom-f
  âˆ˜ Homomorphism.preserve-relations hom-g

import      Data.Tuple as Tuple
open import Function.Equals
open import Function.Equals.Proofs
open import Function.Inverse
open import Lang.Inspect
open import Logic.Predicate.Equiv
open import Structure.Category
open import Structure.Categorical.Properties
open import Structure.Function.Domain.Proofs

instance
  map-function : âˆ€{â„“â‚ â„“â‚‚}{A : Type{â„“â‚}}{B : Type{â„“â‚‚}} â†’ Function â¦ƒ [âŠœ]-equiv â¦„ â¦ƒ [âŠœ]-equiv â¦„ (map{A = A}{B = B}{n = n})
  map-function {A = A}{B = B} = intro proof where
    proof : âˆ€{f g : A â†’ B} â†’ (f âŠœ g) â†’ (map{n = n} f âŠœ map g)
    _âŠœ_.proof (proof p) {âˆ…}     = reflexivity(_â‰¡_)
    _âŠœ_.proof (proof p) {x âŠ° l} = congruenceâ‚‚(_âŠ°_) (_âŠœ_.proof p) (_âŠœ_.proof (proof p) {l})

instance
  Structure-Homomorphism-category : Category(_â†’â‚›â‚œáµ£áµ¤_ {â„“â‚˜})
  Category._âˆ˜_ Structure-Homomorphism-category = _âˆ˜â‚›â‚œáµ£áµ¤_
  Category.id  Structure-Homomorphism-category = idâ‚›â‚œáµ£áµ¤
  BinaryOperator.congruence (Category.binaryOperator Structure-Homomorphism-category) = [âŠœ][âˆ˜]-binaryOperator-raw
  _âŠœ_.proof (Morphism.Associativity.proof (Category.associativity Structure-Homomorphism-category) {_} {_} {_} {_} {[âˆƒ]-intro f} {[âˆƒ]-intro g} {[âˆƒ]-intro h}) {x} = reflexivity(_â‰¡_) {f(g(h(x)))}
  _âŠœ_.proof (Morphism.Identityâ‚—.proof (Tuple.left (Category.identity Structure-Homomorphism-category)) {f = [âˆƒ]-intro f}) {x} = reflexivity(_â‰¡_) {f(x)}
  _âŠœ_.proof (Morphism.Identityáµ£.proof (Tuple.right (Category.identity Structure-Homomorphism-category)) {f = [âˆƒ]-intro f}) {x} = reflexivity(_â‰¡_) {f(x)}

module _ {F@([âˆƒ]-intro f) : _â†’â‚›â‚œáµ£áµ¤_ {â„“â‚˜}{â„“â‚˜} A B} where
  isomorphism-surjective-embedding : Morphism.Isomorphism â¦ƒ [â‰¡âˆƒ]-equiv â¦ƒ [âŠœ]-equiv â¦„ â¦„ (\{A} â†’ _âˆ˜â‚›â‚œáµ£áµ¤_ {A = A})(idâ‚›â‚œáµ£áµ¤)(F) â†” (Surjective(f) Logic.âˆ§ Embedding(A)(B)(f))
  Tuple.left isomorphism-surjective-embedding (Logic.[âˆ§]-intro surj embed) = [âˆƒ]-intro ([âˆƒ]-intro _ â¦ƒ hom â¦„) â¦ƒ Logic.[âˆ§]-intro inverâ‚— inveráµ£ â¦„ where
    fâ»Â¹ = inváµ£-surjective f â¦ƒ surj â¦„
    instance
      inver : Inverse(f)(fâ»Â¹)
      inver = Logic.[âˆ§]-elimáµ£ ([âˆƒ]-proof (bijective-to-invertible â¦ƒ bij = injective-surjective-to-bijective(f)  â¦ƒ Embedding.injection embed â¦„ â¦ƒ surj â¦„ â¦„))

    instance
      hom : Homomorphism(B)(A)(fâ»Â¹)
      Homomorphism.preserve-functions hom {fi = fi} {xs = xs} =
        fâ»Â¹(fn B fi xs)                   ğŸ–[ _â‰¡_ ]-[ congruenceâ‚(fâ»Â¹) (congruenceâ‚(fn B fi) (_âŠœ_.proof map-id)) ]-sym
        fâ»Â¹(fn B fi (map id xs))          ğŸ–[ _â‰¡_ ]-[ congruenceâ‚(fâ»Â¹) (congruenceâ‚(fn B fi) (_âŠœ_.proof (congruenceâ‚(map) (intro (Inverseáµ£.proof(Logic.[âˆ§]-elimáµ£ inver)))) {xs})) ]-sym
        fâ»Â¹(fn B fi (map (f âˆ˜ fâ»Â¹) xs))   ğŸ–[ _â‰¡_ ]-[ congruenceâ‚(fâ»Â¹) (congruenceâ‚(fn B fi) (_âŠœ_.proof map-[âˆ˜] {xs})) ]
        fâ»Â¹(fn B fi (map f (map fâ»Â¹ xs))) ğŸ–[ _â‰¡_ ]-[ congruenceâ‚(fâ»Â¹) (Homomorphism.preserve-functions (Embedding.homomorphism embed)) ]-sym
        fâ»Â¹(f(fn A fi (map fâ»Â¹ xs)))      ğŸ–[ _â‰¡_ ]-[ Inverseâ‚—.proof(Logic.[âˆ§]-elimâ‚— inver) ]
        fn A fi (map fâ»Â¹ xs)              ğŸ–-end

      Homomorphism.preserve-relations hom {ri = ri} {xs = xs} p = Embedding.preserve-relations-converse embed {xs = map fâ»Â¹ xs} (substituteâ‚áµ£(IsTrue âˆ˜ rel B ri) (_âŠœ_.proof proof {xs}) p) where
        proof =
          id                ğŸ–[ _âŠœ_ ]-[ map-id ]-sym
          map id            ğŸ–[ _âŠœ_ ]-[ congruenceâ‚(map) (intro (Inverseáµ£.proof(Logic.[âˆ§]-elimáµ£ inver))) ]-sym
          map(f âˆ˜ fâ»Â¹)      ğŸ–[ _âŠœ_ ]-[ map-[âˆ˜] ]
          (map f âˆ˜ map fâ»Â¹) ğŸ–-end

    inverâ‚— : Morphism.Inverseâ‚— _ _ F ([âˆƒ]-intro fâ»Â¹)
    Morphism.Inverseâ‚—.proof inverâ‚— = intro(Inverseâ‚—.proof(Logic.[âˆ§]-elimâ‚— inver))

    inveráµ£ : Morphism.Inverseáµ£ _ _ F ([âˆƒ]-intro fâ»Â¹)
    Morphism.Inverseáµ£.proof inveráµ£ = intro(Inverseáµ£.proof(Logic.[âˆ§]-elimáµ£ inver))
  Tuple.right isomorphism-surjective-embedding iso = Logic.[âˆ§]-intro infer (intro (\{n}{ri}{xs} â†’ {!proof!})) where
    instance
      bij : Bijective(f)
    instance
      inj : Injective(f)
      inj = bijective-to-injective(f)
    instance
      surj : Surjective(f)
      surj = bijective-to-surjective(f)
    proof : IsTrue(rel A ri xs) â† IsTrue(rel B ri (map f(xs)))
    proof p relation x = {!!}
    proof2 : let _ = (rel A ri xs) in Surjective(f)
    proof2 = {!!}
-- (intro (proof {!!} {!!}))
