module BooleanTheorems where -- TODO: Move

import      Level as Lvl
open import Boolean
open        Boolean.Operators
open import Data
open import Relator.Equals(Lvl.ğŸ)

bivalence : âˆ€{a} â†’ ((a â‰¡ ğ‘‡) â€– (a â‰¡ ğ¹))
bivalence {ğ‘‡} = Either.Left  [â‰¡]-intro
bivalence {ğ¹} = Either.Right [â‰¡]-intro

[âˆ§]-intro-[ğ‘‡] : âˆ€{a b} â†’ (a â‰¡ ğ‘‡) â†’ (b â‰¡ ğ‘‡) â†’ ((a âˆ§ b) â‰¡ ğ‘‡)
[âˆ§]-intro-[ğ‘‡] [â‰¡]-intro [â‰¡]-intro = [â‰¡]-intro

[âˆ¨]-introâ‚—-[ğ‘‡] : âˆ€{a b} â†’ (a â‰¡ ğ‘‡) â†’ ((a âˆ¨ b) â‰¡ ğ‘‡)
[âˆ¨]-introâ‚—-[ğ‘‡] {_}{ğ‘‡} [â‰¡]-intro = [â‰¡]-intro
[âˆ¨]-introâ‚—-[ğ‘‡] {_}{ğ¹} [â‰¡]-intro = [â‰¡]-intro

[âˆ¨]-introáµ£-[ğ‘‡] : âˆ€{a b} â†’ (b â‰¡ ğ‘‡) â†’ ((a âˆ¨ b) â‰¡ ğ‘‡)
[âˆ¨]-introáµ£-[ğ‘‡] {ğ‘‡}{_} [â‰¡]-intro = [â‰¡]-intro
[âˆ¨]-introáµ£-[ğ‘‡] {ğ¹}{_} [â‰¡]-intro = [â‰¡]-intro

[âˆ§]-elim-[ğ‘‡] : âˆ€{a b} â†’ ((a âˆ§ b) â‰¡ ğ‘‡) â†’ (a â‰¡ ğ‘‡)
[âˆ§]-elim-[ğ‘‡] {ğ‘‡}{ğ‘‡} [â‰¡]-intro = [â‰¡]-intro
[âˆ§]-elim-[ğ‘‡] {ğ‘‡}{ğ¹} ()
[âˆ§]-elim-[ğ‘‡] {ğ¹}{ğ‘‡} ()
[âˆ§]-elim-[ğ‘‡] {ğ¹}{ğ¹} ()

[âˆ¨]-elim-[ğ‘‡] : âˆ€{a b c} â†’ ((a â‰¡ ğ‘‡) â†’ (c â‰¡ ğ‘‡)) â†’ ((b â‰¡ ğ‘‡) â†’ (c â‰¡ ğ‘‡)) â†’ ((a âˆ¨ b) â‰¡ ğ‘‡) â†’ (c â‰¡ ğ‘‡)
[âˆ¨]-elim-[ğ‘‡] {ğ‘‡}{ğ‘‡}{_} f _ [â‰¡]-intro = f [â‰¡]-intro
[âˆ¨]-elim-[ğ‘‡] {ğ‘‡}{ğ¹}{_} f _ [â‰¡]-intro = f [â‰¡]-intro
[âˆ¨]-elim-[ğ‘‡] {ğ¹}{ğ‘‡}{_} _ f [â‰¡]-intro = f [â‰¡]-intro
[âˆ¨]-elim-[ğ‘‡] {ğ¹}{ğ¹}{_} _ f ()

[Â¬]-intro-[ğ‘‡] : âˆ€{a} â†’ (a â‰¡ ğ¹) â†’ (Â¬ a â‰¡ ğ‘‡)
[Â¬]-intro-[ğ‘‡] [â‰¡]-intro = [â‰¡]-intro

[Â¬]-elim-[ğ‘‡] : âˆ€{a} â†’ (Â¬ a â‰¡ ğ‘‡) â†’ (a â‰¡ ğ¹)
[Â¬]-elim-[ğ‘‡] {ğ‘‡} ()
[Â¬]-elim-[ğ‘‡] {ğ¹} [â‰¡]-intro = [â‰¡]-intro


[âˆ§]-introâ‚—-[ğ¹] : âˆ€{a b} â†’ (a â‰¡ ğ¹) â†’ ((a âˆ§ b) â‰¡ ğ¹)
[âˆ§]-introâ‚—-[ğ¹] {_}{ğ‘‡} [â‰¡]-intro = [â‰¡]-intro
[âˆ§]-introâ‚—-[ğ¹] {_}{ğ¹} [â‰¡]-intro = [â‰¡]-intro

[âˆ§]-introáµ£-[ğ¹] : âˆ€{a b} â†’ (b â‰¡ ğ¹) â†’ ((a âˆ§ b) â‰¡ ğ¹)
[âˆ§]-introáµ£-[ğ¹] {ğ‘‡}{_} [â‰¡]-intro = [â‰¡]-intro
[âˆ§]-introáµ£-[ğ¹] {ğ¹}{_} [â‰¡]-intro = [â‰¡]-intro

[âˆ¨]-intro-[ğ¹] : âˆ€{a b} â†’ (a â‰¡ ğ¹) â†’ (b â‰¡ ğ¹) â†’ ((a âˆ¨ b) â‰¡ ğ¹)
[âˆ¨]-intro-[ğ¹] [â‰¡]-intro [â‰¡]-intro = [â‰¡]-intro

[Â¬]-intro-[ğ¹] : âˆ€{a} â†’ (Â¬ a â‰¡ ğ‘‡) â†’ (a â‰¡ ğ¹)
[Â¬]-intro-[ğ¹] = [Â¬]-elim-[ğ‘‡]

[Â¬]-elim-[ğ¹] : âˆ€{a} â†’ (a â‰¡ ğ¹) â†’ (Â¬ a â‰¡ ğ‘‡)
[Â¬]-elim-[ğ¹] = [Â¬]-intro-[ğ‘‡]
