module Formalization.LambdaCalculus.SyntaxTransformation where

open import Formalization.LambdaCalculus
open import Functional.Instance
open import Numeral.Natural
open import Numeral.Finite
open import Numeral.Finite.Bound
open import Numeral.Natural.Relation.Order
open import Numeral.Natural.Relation.Order.Proofs
open import Relator.Equals

private variable d dâ‚ dâ‚‚ : â„•
private variable x y : Term(d)

-- Increase the depth level of the given term by something.
-- Example: `depth-[â‰¤](Var(2) : Term(5)) = Var(2) : Term(50)`
depth-[â‰¤] : â¦ƒ _ : (dâ‚ â‰¤ dâ‚‚) â¦„ â†’ Term(dâ‚) â†’ Term(dâ‚‚)
depth-[â‰¤] (Apply t1 t2) = Apply(depth-[â‰¤] t1) (depth-[â‰¤] t2)
depth-[â‰¤] (Abstract t)  = Abstract(depth-[â‰¤] t)
depth-[â‰¤] (Var x)       = Var(bound-[â‰¤] infer x)

-- Increment the depth level of the given term by 1.
-- Example: `depth-ğ’(Var(2) : Term(5)) = Var(2) : Term(6)`
depth-ğ’ : Term(d) â†’ Term(ğ’(d))
depth-ğ’ = depth-[â‰¤]
-- depth-ğ’ (Apply(f)(x))       = Apply (depth-ğ’(f)) (depth-ğ’(x))
-- depth-ğ’ (Abstract(body))    = Abstract(depth-ğ’(body))
-- depth-ğ’ (Var(n))            = Var(bound-ğ’ (n))

Applyâ‚Š : â¦ƒ _ : (dâ‚ â‰¤ dâ‚‚) â¦„ â†’ Term(dâ‚‚) â†’ Term(dâ‚) â†’ Term(dâ‚‚)
Applyâ‚Š {dâ‚}{dâ‚‚} f(x) = Apply f(depth-[â‰¤] {dâ‚}{dâ‚‚} (x))

{-
-- Increase all variables of the given term
var-[â‰¤] : âˆ€{dâ‚ dâ‚‚} â†’ â¦ƒ _ : (dâ‚ â‰¤ dâ‚‚) â¦„ â†’ Term(dâ‚) â†’ Term(dâ‚‚)
var-[â‰¤] (Apply t1 t2) = Apply(depth-[â‰¤] t1) (depth-[â‰¤] t2)
var-[â‰¤] (Abstract t)  = Abstract(depth-[â‰¤] t)
var-[â‰¤] (Var x) = Var({!x + (dâ‚‚ âˆ’ dâ‚)!}) where
  open import Numeral.Natural.TotalOper
-}

-- Increment all variables of the given term.
-- Example: `var-ğ’(Var(2) : Term(5)) = Var(3) : Term(6)`
-- Examples:
--   term : Term(1)
--   term = (1 â†¦ (2 â†¦ 2 â† 2) â† 0 â† 1 â† 0)
--
--   Then:
--   term               = 1 â†¦ (2 â†¦ 2 â† 2) â† 0 â† 1 â† 0
--   var-ğ’(term)        = 2 â†¦ (3 â†¦ 3 â† 3) â† 1 â† 2 â† 1
--   var-ğ’(var-ğ’(term)) = 3 â†¦ (4 â†¦ 4 â† 4) â† 2 â† 3 â† 2
var-ğ’ : Term(d) â†’ Term(ğ’(d))
var-ğ’ (Apply(f)(x))       = Apply (var-ğ’(f)) (var-ğ’(x))
var-ğ’ (Abstract{d}(body)) = Abstract{ğ’(d)} (var-ğ’(body))
var-ğ’ (Var{ğ’(d)}(n))      = Var{ğ’(ğ’(d))} (ğ’(n))

-- Substitutes the most recent free variable with a term in a term, while also decrementing them.
-- `substitute val term` is the term where all occurences in `term` of the outer-most variable is replaced with the term `val`.
-- Examples:
--   substituteOuterVar x (Var(0) : Term(1)) = x
--   substituteOuterVar x ((Apply (Var(1)) (Var(0))) : Term(2)) = Apply (Var(0)) x
--   substituteOuterVar (ğœ† 0 0) ((ğœ† 1 1) â† 0) = ((ğœ† 0 0) â† (ğœ† 0 0))
--   substituteOuterVar (ğœ† 0 0) ((ğœ† 1 1 â† 0) â† 0) = (((ğœ† 0 0) â† (ğœ† 0 0)) â† (ğœ† 0 0))
substituteVar0 : Term(d) â†’ Term(ğ’(d)) â†’ Term(d)
substituteVar0 val (Apply(f)(x))    = Apply (substituteVar0 val f) (substituteVar0 val x)
substituteVar0 val (Abstract(body)) = Abstract (substituteVar0 (var-ğ’ val) body)
substituteVar0 val (Var(ğŸ))         = val
substituteVar0 val (Var(ğ’(v)))      = Var v

{-
substituteMap : (ğ•Ÿ(dâ‚) â†’ Term(dâ‚‚)) â†’ Term(dâ‚) â†’ Term(dâ‚‚)
substituteMap F (Apply(f)(x))    = Apply (substituteMap F (f)) (substituteMap F (x))
substituteMap F (Var(v))         = F(v)
substituteMap F (Abstract(body)) = Abstract (substituteMap F (body)) -- TODO: Probably incorrect
-}

-- Substituting the outer variable of `var-ğ’ x` yields `x`.
-- This is useful because `substituteVar0` uses `var-ğ’` in its definition.
substituteVar0-var-ğ’ : (substituteVar0 y (var-ğ’ x) â‰¡ x)
substituteVar0-var-ğ’ {d}{y}{Apply f x}  rewrite substituteVar0-var-ğ’ {d}{y}{f} rewrite substituteVar0-var-ğ’ {d}{y}{x} = [â‰¡]-intro
substituteVar0-var-ğ’ {d}{y}{Abstract x} rewrite substituteVar0-var-ğ’ {ğ’ d}{var-ğ’ y}{x} = [â‰¡]-intro
substituteVar0-var-ğ’ {_}{_}{Var ğŸ}      = [â‰¡]-intro
substituteVar0-var-ğ’ {_}{_}{Var(ğ’ _)}   = [â‰¡]-intro
{-# REWRITE substituteVar0-var-ğ’ #-}
