module Function.DomainRaise where

open import Data
open import Data.Boolean
import      Functional as Fn
import      Lvl
-- open import Numeral.Finite
-- open import Numeral.Finite.Bound
open import Numeral.Natural
open import Numeral.Natural.Oper.Comparisons
-- open import Numeral.Natural.Oper.Comparisons.Proofs
-- open import Numeral.Natural.Relation.Order
-- open import Numeral.Natural.Relation.Order.Proofs
open import Syntax.Number
open import Type

private variable â„“ â„“â‚ â„“â‚‚ : Lvl.Level
private variable T X Y Z : Type{â„“}
private variable n : â„•

-- Repeated function type like an n-ary operator.
-- Examples:
--   (a â†’Ì‚ b)(0) = (b)
--   (a â†’Ì‚ b)(1) = (a â†’ b)
--   (a â†’Ì‚ b)(2) = (a â†’ a â†’ b)
--   (a â†’Ì‚ b)(3) = (a â†’ a â†’ a â†’ b)
--   (a â†’Ì‚ b)(4) = (a â†’ a â†’ a â†’ a â†’ b)
_â†’Ì‚_ : Type{â„“â‚} â†’ Type{â„“â‚‚} â†’ (n : â„•) â†’ Type{if positive?(n) then (â„“â‚ Lvl.âŠ” â„“â‚‚) else â„“â‚‚}
(A â†’Ì‚ B)(ğŸ)       = B
(A â†’Ì‚ B)(ğ’(ğŸ))    = A â†’ B
(A â†’Ì‚ B)(ğ’(ğ’(n))) = A â†’ (A â†’Ì‚ B)(ğ’(n))

-- Applies the same argument on all arguments.
-- Examples:
--   f : (a â†’Ì‚ b)(5)
--   applyRepeated{0} f(x) = f
--   applyRepeated{1} f(x) = f(x)
--   applyRepeated{2} f(x) = f(x)(x)
--   applyRepeated{3} f(x) = f(x)(x)(x)
--   applyRepeated{2}(applyRepeated{3} f(x)) (y) = f(x)(x)(y)(y)(y)
applyRepeated : let _ = n in (X â†’Ì‚ Y)(n) â†’ (X â†’ Y)
applyRepeated{ğŸ}       f(x) = f
applyRepeated{ğ’(ğŸ)}    f(x) = f(x)
applyRepeated{ğ’(ğ’(n))} f(x) = applyRepeated{ğ’(n)} (f(x)) (x)

{-
  -- Applies arguments from a function.
  -- Almost (not really) like a composition operation.
  -- Examples:
  --   f : (a â†’Ì‚ b)(3)
  --   applyFn f g = f (g(2)) (g(1)) (g(0))
  applyFn : âˆ€{n}{Tâ‚}{Tâ‚‚} â†’ (Tâ‚ â†’Ì‚ Tâ‚‚)(n) â†’ (ğ•Ÿ(n) â†’ Tâ‚) â†’ Tâ‚‚
  applyFn{ğŸ}    f g = f
  applyFn{ğ’(n)} f g = applyFn{n} (f(g(â„•-to-ğ•Ÿ (n) {ğ’(n)} â¦ƒ [<?]-ğ’ {n} â¦„))) (g âˆ˜ (bound-ğ’{n}))

  -- TODO: Examples:
  --   swapReverse {3} f (yâ‚‚) (yâ‚) (yâ‚€)
  --   = swapReverse {2} (f(yâ‚‚)) (yâ‚) (yâ‚€)
  --   = swapReverse {1} (f(yâ‚‚) (yâ‚)) (yâ‚€)
  --   = swapReverse {0} (f(yâ‚‚) (yâ‚) (yâ‚€))
  --   = f(yâ‚‚) (yâ‚) (yâ‚€)
  -- swapReverse : âˆ€{n}{Tâ‚}{Tâ‚‚} â†’ (Tâ‚ â†’Ì‚ Tâ‚‚)(n) â†’ (Tâ‚ â†’Ì‚ Tâ‚‚)(n)
  -- swapReverse {ğŸ}    yâ‚€   = yâ‚€
  -- swapReverse {ğ’(n)} f(yâ‚™) = (swapReverse {n} f) âˆ˜ (f(yâ‚™))

  -- directOp : âˆ€{n}{X}{Y} â†’ ((X â†’ Y) â†’Ì‚ ((X ^ n) â†’ (Y ^ n)))(n)
-}

-- Function composition on a multi-argument function (Like PrimitiveRecursion.Composition).
-- Examples:
--   (f âˆ˜â‚„ g) xâ‚ xâ‚‚ xâ‚ƒ xâ‚„
--   = (f âˆ˜â‚ƒ g xâ‚) xâ‚‚ xâ‚ƒ xâ‚„
--   = (f âˆ˜â‚‚ g xâ‚ xâ‚‚) xâ‚ƒ xâ‚„
--   = (f âˆ˜â‚ g xâ‚ xâ‚‚ xâ‚ƒ) xâ‚„
--   = (f âˆ˜ g xâ‚ xâ‚‚ xâ‚ƒ) xâ‚„
--   = f(g xâ‚ xâ‚‚ xâ‚ƒ xâ‚„)
_âˆ˜_ : let _ = n ; _ = X ; _ = Y ; _ = Z in (Y â†’ Z) â†’ (X â†’Ì‚ Y)(n) â†’ (X â†’Ì‚ Z)(n)
_âˆ˜_ {ğŸ}       = Fn.id
_âˆ˜_ {ğ’(ğŸ)}    = Fn._âˆ˜_
_âˆ˜_ {ğ’(ğ’(n))} = Fn._âˆ˜_ Fn.âˆ˜ (_âˆ˜_) -- (f âˆ˜â‚™â‚Šâ‚‚ g)(x) = f âˆ˜â‚™â‚Šâ‚ g(x)

_âˆ˜[_]_ : let _ = X ; _ = Y ; _ = Z in (Y â†’ Z) â†’ (n : â„•) â†’ (X â†’Ì‚ Y)(n) â†’ (X â†’Ì‚ Z)(n)
f âˆ˜[ n ] g = _âˆ˜_ {n = n} f g

_âˆ˜â‚€_ = _âˆ˜_ {0}
_âˆ˜â‚_ = _âˆ˜_ {1}
_âˆ˜â‚‚_ = _âˆ˜_ {2}
_âˆ˜â‚ƒ_ = _âˆ˜_ {3}
_âˆ˜â‚„_ = _âˆ˜_ {4}
_âˆ˜â‚…_ = _âˆ˜_ {5}
_âˆ˜â‚†_ = _âˆ˜_ {6}
_âˆ˜â‚‡_ = _âˆ˜_ {7}
_âˆ˜â‚ˆ_ = _âˆ˜_ {8}
_âˆ˜â‚‰_ = _âˆ˜_ {9}

-- TODO: Flip the arguments and make n explicit
-- Single function composition on every argument.
-- (f on g)(yâ‚)(yâ‚‚).. = g (f(yâ‚)) (f(yâ‚‚)) ..
-- Examples:
--   _on_ {3} f g (yâ‚‚) (yâ‚) (yâ‚€)
--   = _on_ {2} f (g (f(yâ‚‚))) (yâ‚) (yâ‚€)
--   = _on_ {1} f (g (f(yâ‚‚)) (f(yâ‚))) (yâ‚€)
--   = _on_ {0} f (g (f(yâ‚‚)) (f(yâ‚)) (f(yâ‚€)))
--   = g (f(yâ‚‚)) (f(yâ‚)) (f(yâ‚€))
_on_ : let _ = n ; _ = X ; _ = Y ; _ = Z in (Y â†’Ì‚ Z)(n) â†’ (X â†’ Y) â†’ (X â†’Ì‚ Z)(n)
_on_ {n = ğŸ}               = Fn.const
_on_ {n = ğ’(ğŸ)}            = Fn._âˆ˜_
_on_ {n = ğ’(ğ’(n))} f g(yâ‚™) = _on_ {n = ğ’(n)} (f(g(yâ‚™))) g

-- applyOnFn : âˆ€{n}{X}{Y} â†’ (Y â†’Ì‚ Y)(n) â†’ ((X â†’ Y) â†’Ì‚ (X â†’ Y))(n)
-- applyOnFn

-- Constructs a left-associated n-ary operator from a binary operator.
-- Example:
--   naryâ‚—{3} (_â–«_) xâ‚ xâ‚‚ xâ‚ƒ xâ‚„ xâ‚…
--   = ((naryâ‚—{2} (_â–«_)) Fn.âˆ˜ (xâ‚ â–«_)) xâ‚‚ xâ‚ƒ xâ‚„
--   = (naryâ‚—{2} (_â–«_) (xâ‚ â–« xâ‚‚)) xâ‚ƒ xâ‚„ xâ‚…
--   = ((naryâ‚—{1} (_â–«_)) Fn.âˆ˜ ((xâ‚ â–« xâ‚‚) â–«_)) xâ‚ƒ xâ‚„ xâ‚…
--   = (naryâ‚—{1} (_â–«_) ((xâ‚ â–« xâ‚‚) â–« xâ‚ƒ)) xâ‚„ xâ‚…
--   = ((naryâ‚—{0} (_â–«_)) Fn.âˆ˜ (((xâ‚ â–« xâ‚‚) â–« xâ‚ƒ) â–«_)) xâ‚ƒ xâ‚„ xâ‚…
--   = (naryâ‚—{0} (_â–«_) (((xâ‚ â–« xâ‚‚) â–« xâ‚ƒ) â–« xâ‚„)) xâ‚…
--   = ((_â–«_) (((xâ‚ â–« xâ‚‚) â–« xâ‚ƒ) â–« xâ‚„)) xâ‚…
--   = ((((xâ‚ â–« xâ‚‚) â–« xâ‚ƒ) â–« xâ‚„) â–«_) xâ‚…
--   = (((xâ‚ â–« xâ‚‚) â–« xâ‚ƒ) â–« xâ‚„) xâ‚…
naryâ‚— : (n : â„•) â†’ (X â†’ X â†’ X) â†’ (X â†’Ì‚ X)(ğ’(ğ’(n)))
naryâ‚—(ğŸ)    (_â–«_)   = (_â–«_)
naryâ‚—(ğ’(n)) (_â–«_) x = (naryâ‚—(n) (_â–«_)) Fn.âˆ˜ (x â–«_)

-- Constructs a right-associated n-ary operator from a binary operator.
-- Example:
--   naryáµ£{3} (_â–«_) xâ‚ xâ‚‚ xâ‚ƒ xâ‚„ xâ‚…
--   = ((xâ‚ â–«_) âˆ˜[ 4 ] (naryáµ£{2} (_â–«_))) xâ‚‚ xâ‚ƒ xâ‚„ xâ‚…
--   = xâ‚ â–« (naryáµ£{2} (_â–«_) xâ‚‚ xâ‚ƒ xâ‚„ xâ‚…)
--   = xâ‚ â–« (((xâ‚‚ â–«_) âˆ˜[ 3 ] (naryáµ£{1} (_â–«_))) xâ‚ƒ xâ‚„ xâ‚…)
--   = xâ‚ â–« (xâ‚‚ â–« (naryáµ£{1} (_â–«_) xâ‚ƒ xâ‚„ xâ‚…))
--   = xâ‚ â–« (xâ‚‚ â–« (((xâ‚ƒ â–«_) âˆ˜[ 2 ] (naryáµ£{0} (_â–«_))) xâ‚„ xâ‚…))
--   = xâ‚ â–« (xâ‚‚ â–« (xâ‚ƒ â–« (naryáµ£{0} (_â–«_) xâ‚„ xâ‚…)))
--   = xâ‚ â–« (xâ‚‚ â–« (xâ‚ƒ â–« ((_â–«_) xâ‚„ xâ‚…)))
--   = xâ‚ â–« (xâ‚‚ â–« (xâ‚ƒ â–« (xâ‚„ â–« xâ‚…)))
naryáµ£ : (n : â„•) â†’ (X â†’ X â†’ X) â†’ (X â†’Ì‚ X)(ğ’(ğ’(n)))
naryáµ£(ğŸ)    (_â–«_)   = (_â–«_)
naryáµ£(ğ’(n)) (_â–«_) x = (x â–«_) âˆ˜[ ğ’(ğ’(n)) ] (naryáµ£(n) (_â–«_))
