module Numeral.Sign.Proofs where

open import Logic.IntroInstances
open import Numeral.Sign
open import Numeral.Sign.Oper
open import Numeral.Sign.Oper0 renaming (_+_ to _+â‚€_ ; _â¨¯_ to _â¨¯â‚€_ ; âˆ’_ to âˆ’â‚€_)
open import Relator.Equals
open import Relator.Equals.Proofs.Equivalence
open import Structure.Function.Domain
open import Structure.Operator.Properties
open import Structure.Setoid hiding (_â‰¢_)

instance
  [âˆ’|+]-equiv : Equiv(âˆ’|+)
  [âˆ’|+]-equiv = [â‰¡]-equiv

instance
  [âˆ’|0|+]-equiv : Equiv(âˆ’|0|+)
  [âˆ’|0|+]-equiv = [â‰¡]-equiv

instance
  [+]-commutativity : Commutativity(_+_)
  Commutativity.proof [+]-commutativity {â•} {â•} = [â‰¡]-intro
  Commutativity.proof [+]-commutativity {â•} {â–} = [â‰¡]-intro
  Commutativity.proof [+]-commutativity {â–} {â•} = [â‰¡]-intro
  Commutativity.proof [+]-commutativity {â–} {â–} = [â‰¡]-intro

instance
  [â¨¯]-commutativity : Commutativity(_â¨¯_)
  Commutativity.proof [â¨¯]-commutativity {â•} {â•} = [â‰¡]-intro
  Commutativity.proof [â¨¯]-commutativity {â•} {â–} = [â‰¡]-intro
  Commutativity.proof [â¨¯]-commutativity {â–} {â•} = [â‰¡]-intro
  Commutativity.proof [â¨¯]-commutativity {â–} {â–} = [â‰¡]-intro

instance
  [+â‚€]-identityâ‚— : Identityâ‚—(_+â‚€_)(ğŸ)
  Identityâ‚—.proof [+â‚€]-identityâ‚— {â•} = [â‰¡]-intro
  Identityâ‚—.proof [+â‚€]-identityâ‚— {ğŸ} = [â‰¡]-intro
  Identityâ‚—.proof [+â‚€]-identityâ‚— {â–} = [â‰¡]-intro

instance
  [+â‚€]-identityáµ£ : Identityáµ£(_+â‚€_)(ğŸ)
  Identityáµ£.proof [+â‚€]-identityáµ£ {â•} = [â‰¡]-intro
  Identityáµ£.proof [+â‚€]-identityáµ£ {ğŸ} = [â‰¡]-intro
  Identityáµ£.proof [+â‚€]-identityáµ£ {â–} = [â‰¡]-intro

instance
  [+â‚€]-identity : Identity(_+â‚€_)(ğŸ)
  [+â‚€]-identity = intro

instance
  [+â‚€]-inverseFunctionâ‚— : InverseFunctionâ‚—(_+â‚€_)(âˆ’â‚€_)
  InverseFunctionâ‚—.proof [+â‚€]-inverseFunctionâ‚— {â•} = [â‰¡]-intro
  InverseFunctionâ‚—.proof [+â‚€]-inverseFunctionâ‚— {ğŸ} = [â‰¡]-intro
  InverseFunctionâ‚—.proof [+â‚€]-inverseFunctionâ‚— {â–} = [â‰¡]-intro

instance
  [+â‚€]-inverseFunctionáµ£ : InverseFunctionáµ£(_+â‚€_)(âˆ’â‚€_)
  InverseFunctionáµ£.proof [+â‚€]-inverseFunctionáµ£ {â•} = [â‰¡]-intro
  InverseFunctionáµ£.proof [+â‚€]-inverseFunctionáµ£ {ğŸ} = [â‰¡]-intro
  InverseFunctionáµ£.proof [+â‚€]-inverseFunctionáµ£ {â–} = [â‰¡]-intro

instance
  [+â‚€]-inverseFunction : InverseFunction(_+â‚€_)(âˆ’â‚€_)
  [+â‚€]-inverseFunction = intro

instance
  [â¨¯â‚€]-commutativity : Commutativity(_â¨¯â‚€_)
  Commutativity.proof [â¨¯â‚€]-commutativity {â•} {â•} = [â‰¡]-intro
  Commutativity.proof [â¨¯â‚€]-commutativity {â•} {ğŸ} = [â‰¡]-intro
  Commutativity.proof [â¨¯â‚€]-commutativity {â•} {â–} = [â‰¡]-intro
  Commutativity.proof [â¨¯â‚€]-commutativity {ğŸ} {â•} = [â‰¡]-intro
  Commutativity.proof [â¨¯â‚€]-commutativity {ğŸ} {ğŸ} = [â‰¡]-intro
  Commutativity.proof [â¨¯â‚€]-commutativity {ğŸ} {â–} = [â‰¡]-intro
  Commutativity.proof [â¨¯â‚€]-commutativity {â–} {â•} = [â‰¡]-intro
  Commutativity.proof [â¨¯â‚€]-commutativity {â–} {ğŸ} = [â‰¡]-intro
  Commutativity.proof [â¨¯â‚€]-commutativity {â–} {â–} = [â‰¡]-intro

instance
  [â¨¯â‚€]-associativity : Associativity(_â¨¯â‚€_)
  Associativity.proof [â¨¯â‚€]-associativity {â•} {â•} {â•} = [â‰¡]-intro
  Associativity.proof [â¨¯â‚€]-associativity {â•} {â•} {ğŸ} = [â‰¡]-intro
  Associativity.proof [â¨¯â‚€]-associativity {â•} {â•} {â–} = [â‰¡]-intro
  Associativity.proof [â¨¯â‚€]-associativity {â•} {ğŸ} {â•} = [â‰¡]-intro
  Associativity.proof [â¨¯â‚€]-associativity {â•} {ğŸ} {ğŸ} = [â‰¡]-intro
  Associativity.proof [â¨¯â‚€]-associativity {â•} {ğŸ} {â–} = [â‰¡]-intro
  Associativity.proof [â¨¯â‚€]-associativity {â•} {â–} {â•} = [â‰¡]-intro
  Associativity.proof [â¨¯â‚€]-associativity {â•} {â–} {ğŸ} = [â‰¡]-intro
  Associativity.proof [â¨¯â‚€]-associativity {â•} {â–} {â–} = [â‰¡]-intro
  Associativity.proof [â¨¯â‚€]-associativity {ğŸ} {â•} {â•} = [â‰¡]-intro
  Associativity.proof [â¨¯â‚€]-associativity {ğŸ} {â•} {ğŸ} = [â‰¡]-intro
  Associativity.proof [â¨¯â‚€]-associativity {ğŸ} {â•} {â–} = [â‰¡]-intro
  Associativity.proof [â¨¯â‚€]-associativity {ğŸ} {ğŸ} {â•} = [â‰¡]-intro
  Associativity.proof [â¨¯â‚€]-associativity {ğŸ} {ğŸ} {ğŸ} = [â‰¡]-intro
  Associativity.proof [â¨¯â‚€]-associativity {ğŸ} {ğŸ} {â–} = [â‰¡]-intro
  Associativity.proof [â¨¯â‚€]-associativity {ğŸ} {â–} {â•} = [â‰¡]-intro
  Associativity.proof [â¨¯â‚€]-associativity {ğŸ} {â–} {ğŸ} = [â‰¡]-intro
  Associativity.proof [â¨¯â‚€]-associativity {ğŸ} {â–} {â–} = [â‰¡]-intro
  Associativity.proof [â¨¯â‚€]-associativity {â–} {â•} {â•} = [â‰¡]-intro
  Associativity.proof [â¨¯â‚€]-associativity {â–} {â•} {ğŸ} = [â‰¡]-intro
  Associativity.proof [â¨¯â‚€]-associativity {â–} {â•} {â–} = [â‰¡]-intro
  Associativity.proof [â¨¯â‚€]-associativity {â–} {ğŸ} {â•} = [â‰¡]-intro
  Associativity.proof [â¨¯â‚€]-associativity {â–} {ğŸ} {ğŸ} = [â‰¡]-intro
  Associativity.proof [â¨¯â‚€]-associativity {â–} {ğŸ} {â–} = [â‰¡]-intro
  Associativity.proof [â¨¯â‚€]-associativity {â–} {â–} {â•} = [â‰¡]-intro
  Associativity.proof [â¨¯â‚€]-associativity {â–} {â–} {ğŸ} = [â‰¡]-intro
  Associativity.proof [â¨¯â‚€]-associativity {â–} {â–} {â–} = [â‰¡]-intro

instance
  [â¨¯â‚€]-absorberâ‚— : Absorberâ‚—(_â¨¯â‚€_)(ğŸ)
  Absorberâ‚—.proof [â¨¯â‚€]-absorberâ‚— {â•} = [â‰¡]-intro
  Absorberâ‚—.proof [â¨¯â‚€]-absorberâ‚— {ğŸ} = [â‰¡]-intro
  Absorberâ‚—.proof [â¨¯â‚€]-absorberâ‚— {â–} = [â‰¡]-intro

instance
  [â¨¯â‚€]-absorberáµ£ : Absorberáµ£(_â¨¯â‚€_)(ğŸ)
  Absorberáµ£.proof [â¨¯â‚€]-absorberáµ£ {â•} = [â‰¡]-intro
  Absorberáµ£.proof [â¨¯â‚€]-absorberáµ£ {ğŸ} = [â‰¡]-intro
  Absorberáµ£.proof [â¨¯â‚€]-absorberáµ£ {â–} = [â‰¡]-intro

instance
  [â¨¯â‚€]-absorber : Absorber(_â¨¯â‚€_)(ğŸ)
  [â¨¯â‚€]-absorber = intro

instance
  [âˆ’]-involution : Involution(âˆ’_)
  Involution.proof [âˆ’]-involution {â•} = [â‰¡]-intro
  Involution.proof [âˆ’]-involution {â–} = [â‰¡]-intro

[âˆ’]-no-fixpoints : âˆ€{s} â†’ (âˆ’ s â‰¢ s)
[âˆ’]-no-fixpoints {â•} ()
[âˆ’]-no-fixpoints {â–} ()
