module Functional.Raise where

open import Functional
import NaturalNumbers as Nat

_â° : âˆ€ {n} {T : Set n} â†’ (T â†’ T) â†’ (T â†’ T)
_â° = id

_Â¹ : âˆ€ {n} {T : Set n} â†’ (T â†’ T) â†’ (T â†’ T)
_Â¹ f = f

_Â² : âˆ€ {n} {T : Set n} â†’ (T â†’ T) â†’ (T â†’ T)
_Â² f = f âˆ˜ f

_Â³ : âˆ€ {n} {T : Set n} â†’ (T â†’ T) â†’ (T â†’ T)
_Â³ f = f âˆ˜ f âˆ˜ f

_â´ : âˆ€ {n} {T : Set n} â†’ (T â†’ T) â†’ (T â†’ T)
_â´ f = f âˆ˜ f âˆ˜ f âˆ˜ f

_âµ : âˆ€ {n} {T : Set n} â†’ (T â†’ T) â†’ (T â†’ T)
_âµ f = f âˆ˜ f âˆ˜ f âˆ˜ f âˆ˜ f

_â¶ : âˆ€ {n} {T : Set n} â†’ (T â†’ T) â†’ (T â†’ T)
_â¶ f = f âˆ˜ f âˆ˜ f âˆ˜ f âˆ˜ f âˆ˜ f

_â· : âˆ€ {n} {T : Set n} â†’ (T â†’ T) â†’ (T â†’ T)
_â· f = f âˆ˜ f âˆ˜ f âˆ˜ f âˆ˜ f âˆ˜ f âˆ˜ f

_â¸ : âˆ€ {n} {T : Set n} â†’ (T â†’ T) â†’ (T â†’ T)
_â¸ f = f âˆ˜ f âˆ˜ f âˆ˜ f âˆ˜ f âˆ˜ f âˆ˜ f âˆ˜ f

_â¹ : âˆ€ {n} {T : Set n} â†’ (T â†’ T) â†’ (T â†’ T)
_â¹ f = f âˆ˜ f âˆ˜ f âˆ˜ f âˆ˜ f âˆ˜ f âˆ˜ f âˆ˜ f âˆ˜ f

_^_ : âˆ€ {n} {T : Set n} â†’ (T â†’ T) â†’ Nat.â„• â†’ (T â†’ T)
_^_ f Nat.â„•0 = id
_^_ f (Nat.ð‘†(n)) = f âˆ˜ (f ^ n)

repeatâ‚— : âˆ€ {n} {X Y : Set n} â†’ Nat.â„• â†’ Y â†’ (Y â†’ X â†’ Y) â†’ X â†’ Y
repeatâ‚— Nat.â„•0 null op elem = null
repeatâ‚— (Nat.ð‘†(n)) null op elem = op (repeatâ‚— n null op elem) elem
-- Example: repeatâ‚— 3 id (_âˆ˜_) f = ((id âˆ˜ f) âˆ˜ f) âˆ˜ f
-- Example in Haskell: (foldl (.) (id) (take 5 (repeat f)))
-- in Haskell: (\n null op elem -> foldl op null (take n (repeat elem))) :: Int -> a -> (b -> a -> b) -> b -> b

repeatáµ£ : âˆ€ {n} {X Y : Set n} â†’ Nat.â„• â†’ X â†’ (X â†’ Y â†’ Y) â†’ Y â†’ Y
repeatáµ£ Nat.â„•0 elem op null = null
repeatáµ£ (Nat.ð‘†(n)) elem op null = op elem (repeatáµ£ n elem op null)
-- in Haskell: (\n elem op null -> foldr op null (take n (repeat elem))) :: Int -> a -> (a -> b -> b) -> b -> b

-- TODO: curry âˆ˜ curry does not work with repeat because LHSâ‰ RHS, but can this be fixed?
-- curry             :: ((a, b) -> c) -> a -> b -> c
-- curry.curry       :: (((a, b), b1) -> c) -> a -> b -> b1 -> c
-- curry.curry.curry :: ((((a, b), b1), b2) -> c) -> a -> b -> b1 -> b2 -> c
