module Numeral.Natural.Relation.Order.Proofs where

import Lvl
open import Data.Tuple as Tuple using (_â¨¯_ ; _,_)
open import Functional
open import Logic
open import Logic.Propositional
open import Logic.Propositional.Theorems
open import Logic.Predicate
open import Numeral.Natural
open import Numeral.Natural.Oper
open import Numeral.Natural.Oper.Proofs
open import Numeral.Natural.Induction
open import Numeral.Natural.Relation.Order
open import Relator.Equals
open import Relator.Equals.Proofs
import      Structure.Relator.Names as Names
open import Structure.Operator.Properties
open import Structure.Relator.Ordering
open import Structure.Relator.Properties
open import Syntax.Transitivity
open import Type

-- TODO: A method for pattern matching: https://stackoverflow.com/questions/20682013/agda-why-am-i-unable-to-pattern-match-on-refl

[<]-minimum : âˆ€{x : â„•} â†’ (0 < ğ’(x))
[<]-minimum {x} = [â‰¤]-with-[ğ’] {0} â¦ƒ [â‰¤]-minimum â¦„

[â‰¡]-to-[â‰¤] : âˆ€{x y : â„•} â†’ (x â‰¡ y) â†’ (x â‰¤ y)
[â‰¡]-to-[â‰¤] {ğŸ}   {_}    ([â‰¡]-intro) = [â‰¤]-minimum
[â‰¡]-to-[â‰¤] {ğ’(x)}{ğ’(y)} ([â‰¡]-intro) = [â‰¤]-with-[ğ’] â¦ƒ [â‰¡]-to-[â‰¤] {x}{y} ([â‰¡]-intro) â¦„

[â‰¡]-to-[â‰¥] : âˆ€{x y : â„•} â†’ (x â‰¡ y) â†’ (x â‰¥ y)
[â‰¡]-to-[â‰¥] = [â‰¡]-to-[â‰¤] âˆ˜ symmetry(_â‰¡_)

[â‰°]-to-[â‰¢] : âˆ€{x y : â„•} â†’ (x â‰° y) â†’ (x â‰¢ y)
[â‰°]-to-[â‰¢] = contrapositiveáµ£ [â‰¡]-to-[â‰¤]

[â‰±]-to-[â‰¢] : âˆ€{x y : â„•} â†’ (x â‰± y) â†’ (x â‰¢ y)
[â‰±]-to-[â‰¢] = contrapositiveáµ£ [â‰¡]-to-[â‰¥]

[â‰¤][0]áµ£ : âˆ€{x : â„•} â†’ (x â‰¤ 0) â†’ (x â‰¡ 0)
[â‰¤][0]áµ£ {ğŸ}    (_) = [â‰¡]-intro
[â‰¤][0]áµ£ {ğ’(_)} ()

[â‰¤][0]áµ£-negation : âˆ€{x : â„•} â†’ (ğ’(x) â‰° 0)
[â‰¤][0]áµ£-negation ()

[â‰¤]-successor : âˆ€{x y : â„•} â†’ (x â‰¤ y) â†’ (x â‰¤ ğ’(y))
[â‰¤]-successor {ğŸ}   {_}    (_) = [â‰¤]-minimum
[â‰¤]-successor {ğ’(x)}{ğŸ}    ()
[â‰¤]-successor {ğ’(x)}{ğ’(y)} ([â‰¤]-with-[ğ’] â¦ƒ proof â¦„) = [â‰¤]-with-[ğ’] â¦ƒ [â‰¤]-successor {x}{y} (proof) â¦„

[â‰¤]-predecessor : âˆ€{x y : â„•} â†’ (ğ’(x) â‰¤ y) â†’ (x â‰¤ y)
[â‰¤]-predecessor {x}   {ğŸ}    ()
[â‰¤]-predecessor {ğŸ}   {ğ’(y)} (_) = [â‰¤]-minimum
[â‰¤]-predecessor {ğ’(x)}{ğ’(y)} ([â‰¤]-with-[ğ’] â¦ƒ proof â¦„) = [â‰¤]-with-[ğ’] â¦ƒ [â‰¤]-predecessor {x}{y} (proof) â¦„

[â‰¤]-without-[ğ’] : âˆ€{x y : â„•} â†’ (ğ’(x) â‰¤ ğ’(y)) â†’ (x â‰¤ y)
[â‰¤]-without-[ğ’] ([â‰¤]-with-[ğ’] â¦ƒ proof â¦„) = proof

[â‰¤][ğ’]â‚— : âˆ€{x : â„•} â†’ Â¬(ğ’(x) â‰¤ x)
[â‰¤][ğ’]â‚— {ğŸ}    (1â‰¤0)    = [â‰¤][0]áµ£-negation{0}(1â‰¤0)
[â‰¤][ğ’]â‚— {ğ’(n)} (SSnâ‰¤Sn) = [â‰¤][ğ’]â‚— {n} ([â‰¤]-without-[ğ’] {ğ’(n)}{n} (SSnâ‰¤Sn))

instance
  [â‰¤]-reflexivity : Reflexivity (_â‰¤_)
  Reflexivity.proof([â‰¤]-reflexivity) = [â‰¡]-to-[â‰¤] [â‰¡]-intro

instance
  [â‰¤]-transitivity : Transitivity (_â‰¤_)
  Transitivity.proof([â‰¤]-transitivity) = proof where
    proof : Names.Transitivity (_â‰¤_)
    proof {ğŸ}   {_}   {_} (_)(_) = [â‰¤]-minimum
    proof {ğ’(a)}{ğ’(b)}{ğ’(c)} ([â‰¤]-with-[ğ’] â¦ƒ proofâ‚— â¦„) ([â‰¤]-with-[ğ’] â¦ƒ proofáµ£ â¦„ ) =
      [â‰¤]-with-[ğ’] â¦ƒ proof {a}{b}{c} (proofâ‚—) (proofáµ£) â¦„

instance
  [â‰¤]-antisymmetry : Antisymmetry (_â‰¤_) (_â‰¡_)
  Antisymmetry.proof([â‰¤]-antisymmetry) = proof where
    proof : Names.Antisymmetry (_â‰¤_) (_â‰¡_)
    proof {ğŸ}    {ğŸ}    (_) (_) = [â‰¡]-intro
    proof {ğ’(_)} {ğŸ}    ()
    proof {ğŸ}    {ğ’(_)} (_) ()
    proof {ğ’(a)} {ğ’(b)} ([â‰¤]-with-[ğ’] â¦ƒ proofâ‚— â¦„) ([â‰¤]-with-[ğ’] â¦ƒ proofáµ£ â¦„) =
      [â‰¡]-with(ğ’) (proof {a}{b} proofâ‚— proofáµ£)

instance
  [â‰¤]-totality : ConverseTotal(_â‰¤_)
  ConverseTotal.proof([â‰¤]-totality) = proof where
    proof : Names.ConverseTotal(_â‰¤_)
    proof {ğŸ}   {ğŸ}    = [âˆ¨]-introâ‚— ([â‰¡]-to-[â‰¤] [â‰¡]-intro)
    proof {ğ’(a)}{ğŸ}    = [âˆ¨]-introáµ£ ([â‰¤]-minimum)
    proof {ğŸ}   {ğ’(b)} = [âˆ¨]-introâ‚— ([â‰¤]-minimum)
    proof {ğ’(a)}{ğ’(b)} = [âˆ¨]-elim ([âˆ¨]-introâ‚— âˆ˜ (proof â†¦ [â‰¤]-with-[ğ’] {a}{b} â¦ƒ proof â¦„)) ([âˆ¨]-introáµ£ âˆ˜ (proof â†¦ [â‰¤]-with-[ğ’] {b}{a} â¦ƒ proof â¦„)) (proof {a}{b})

instance
  [â‰¤]-weakPartialOrder : Weak.PartialOrder (_â‰¤_) (_â‰¡_)
  [â‰¤]-weakPartialOrder = record{}

instance
  [â‰¤]-weakTotalOrder : Weak.TotalOrder (_â‰¤_) (_â‰¡_)
  [â‰¤]-weakTotalOrder = record{}

instance
  [â‰¥]-reflexivity : Reflexivity (_â‰¥_)
  Reflexivity.proof([â‰¥]-reflexivity) = Reflexivity.proof([â‰¤]-reflexivity)

instance
  [â‰¥]-transitivity : Transitivity (_â‰¥_)
  Transitivity.proof([â‰¥]-transitivity) = swap(Transitivity.proof([â‰¤]-transitivity))

instance
  [â‰¥]-antisymmetry : Antisymmetry (_â‰¥_) (_â‰¡_)
  Antisymmetry.proof([â‰¥]-antisymmetry) = swap(Antisymmetry.proof([â‰¤]-antisymmetry))

instance
  [â‰¥]-totality : ConverseTotal(_â‰¥_)
  ConverseTotal.proof([â‰¥]-totality) = ConverseTotal.proof([â‰¤]-totality)

instance
  [â‰¥]-weakPartialOrder : Weak.PartialOrder (_â‰¥_) (_â‰¡_)
  [â‰¥]-weakPartialOrder = record{}

instance
  [â‰¥]-weakTotalOrder : Weak.TotalOrder (_â‰¥_) (_â‰¡_)
  [â‰¥]-weakTotalOrder = record{}

[â‰¥]-to-[â‰®] : âˆ€{a b : â„•} â†’ (a â‰® b) â† (a â‰¥ b)
[â‰¥]-to-[â‰®] {a}{b} (bâ‰¤a) (ğ’aâ‰¤b) = [â‰¤][ğ’]â‚— (transitivity(_â‰¤_) {ğ’(a)}{b}{a} (ğ’aâ‰¤b) (bâ‰¤a))

[â‰¤]-to-[â‰¯] : âˆ€{a b : â„•} â†’ (a â‰¯ b) â† (a â‰¤ b)
[â‰¤]-to-[â‰¯] {a}{b} (aâ‰¤b) (ğ’bâ‰¤a) = [â‰¥]-to-[â‰®] {b}{a} (aâ‰¤b) (ğ’bâ‰¤a)

[>]-to-[â‰°] : âˆ€{a b : â„•} â†’ (a â‰° b) â† (a > b)
[>]-to-[â‰°] {a}{b} (ğ’bâ‰¤a) (aâ‰¤b) = [â‰¤]-to-[â‰¯] (aâ‰¤b) (ğ’bâ‰¤a)

[<]-to-[â‰±] : âˆ€{a b : â„•} â†’ (a â‰± b) â† (a < b)
[<]-to-[â‰±] {a}{b} (ğ’aâ‰¤b) (bâ‰¤a) = [â‰¥]-to-[â‰®] (bâ‰¤a) (ğ’aâ‰¤b)

[<][0]áµ£ : âˆ€{x : â„•} â†’ (x â‰® 0)
[<][0]áµ£ = [â‰¤][0]áµ£-negation

instance
  [<]-irreflexivity : Irreflexivity (_<_)
  Irreflexivity.proof([<]-irreflexivity) = [â‰¤][ğ’]â‚—

instance
  [<]-transitivity : Transitivity (_<_)
  Transitivity.proof([<]-transitivity) {x}{y}{z} (l) (r) = Transitivity.proof([â‰¤]-transitivity) {ğ’(x)} {ğ’(y)} {z} ([â‰¤]-successor (l)) (r)

instance
  [<]-asymmetry : Asymmetry (_<_)
  Asymmetry.proof([<]-asymmetry) (l) (r) = Irreflexivity.proof([<]-irreflexivity) (Transitivity.proof([<]-transitivity) (l) (r))

instance
  [<]-strictOrder : Strict.PartialOrder (_<_)
  [<]-strictOrder = record{}

instance
  [>]-irreflexivity : Irreflexivity (_>_)
  Irreflexivity.proof([>]-irreflexivity) = Irreflexivity.proof([<]-irreflexivity)

instance
  [>]-transitivity : Transitivity (_>_)
  Transitivity.proof([>]-transitivity) = swap(Transitivity.proof([<]-transitivity))

instance
  [>]-asymmetry : Asymmetry (_>_)
  Asymmetry.proof([>]-asymmetry) = swap(Asymmetry.proof([<]-asymmetry))

instance
  [>]-strictOrder : Strict.PartialOrder (_>_)
  [>]-strictOrder = record{}

[<]-of-[ğ’] : âˆ€{x : â„•} â†’ (x < ğ’(x))
[<]-of-[ğ’] = reflexivity(_â‰¤_)

[<]-of-[ğŸ][ğ’] : âˆ€{x : â„•} â†’ (ğŸ < ğ’(x))
[<]-of-[ğŸ][ğ’] {ğŸ} = [<]-of-[ğ’]
[<]-of-[ğŸ][ğ’] {ğ’ x} = [â‰¤]-with-[ğ’] â¦ƒ [â‰¤]-minimum â¦„

instance
  [â‰¤]-of-[ğ’] : âˆ€{x : â„•} â†’ (x â‰¤ ğ’(x))
  [â‰¤]-of-[ğ’] = [â‰¤]-successor(reflexivity(_â‰¤_))

[<][â‰¢]-equivalence : âˆ€{x} â†’ (x > 0) â†” (x â‰¢ 0)
[<][â‰¢]-equivalence {x} = [â†”]-intro (l{x}) (r{x}) where
  l : âˆ€{x} â†’ (x > 0) â† (x â‰¢ 0)
  l{ğŸ}    (xâ‰¢ğŸ)  = [âŠ¥]-elim((xâ‰¢ğŸ)([â‰¡]-intro))
  l{ğ’(x)} (ğ’xâ‰¢ğŸ) = [â‰¤]-with-[ğ’] â¦ƒ [â‰¤]-minimum â¦„

  r : âˆ€{x} â†’ (x > 0) â†’ (x â‰¢ 0)
  r{ğŸ}    ()
  r{ğ’(x)} (ğŸâ‰¤ğ’x) (ğ’xâ‰¡ğŸ) with [â‰¡]-substitutionáµ£ (ğ’xâ‰¡ğŸ) {expr â†¦ 1 â‰¤ expr} (ğŸâ‰¤ğ’x)
  ... | ()

 -- [â‰¤]-with-[ğ’]

[â‰¤]-to-[<][â‰¡] : âˆ€{a b : â„•} â†’ (a â‰¤ b) â†’ (a < b)âˆ¨(a â‰¡ b)
[â‰¤]-to-[<][â‰¡] {ğŸ}   {ğŸ}    ([â‰¤]-minimum)    = [âˆ¨]-introáµ£([â‰¡]-intro)
[â‰¤]-to-[<][â‰¡] {ğŸ}   {ğ’(b)} ([â‰¤]-minimum)    = [âˆ¨]-introâ‚—([<]-minimum)
[â‰¤]-to-[<][â‰¡] {ğ’(a)}{ğ’(b)} ([â‰¤]-with-[ğ’] â¦ƒ aâ‰¤b â¦„) with [â‰¤]-to-[<][â‰¡] {a}{b} (aâ‰¤b)
... | [âˆ¨]-introâ‚—(a<b) = [âˆ¨]-introâ‚—([â‰¤]-with-[ğ’] â¦ƒ a<b â¦„)
... | [âˆ¨]-introáµ£(aâ‰¡b) = [âˆ¨]-introáµ£([â‰¡]-with(ğ’) (aâ‰¡b))

[â‰®][â‰¢]-to-[â‰°] : âˆ€{a b : â„•} â†’ (a â‰® b) â†’ (a â‰¢ b) â†’ (a â‰° b)
[â‰®][â‰¢]-to-[â‰°] (aâ‰®b) (aâ‰¢b) (aâ‰¤b) with [â‰¤]-to-[<][â‰¡] (aâ‰¤b)
... | [âˆ¨]-introâ‚— (a<b) = aâ‰®b a<b
... | [âˆ¨]-introáµ£ (aâ‰¡b) = aâ‰¢b aâ‰¡b

[<][â‰¡]-to-[â‰¤] : âˆ€{a b : â„•} â†’ (a < b)âˆ¨(a â‰¡ b) â†’ (a â‰¤ b)
[<][â‰¡]-to-[â‰¤] {a}   {.a}   ([âˆ¨]-introáµ£([â‰¡]-intro)) = [â‰¡]-to-[â‰¤] ([â‰¡]-intro)
[<][â‰¡]-to-[â‰¤] {a}   {b}    ([âˆ¨]-introâ‚—(a<b))       = [â‰¤]-predecessor (a<b)

[<]-to-[â‰¤] : âˆ€{a b : â„•} â†’ (a < b) â†’ (a â‰¤ b)
[<]-to-[â‰¤] = [â‰¤]-predecessor

[â‰°]-to-[â‰®] : âˆ€{x y : â„•} â†’ (x â‰° y) â†’ (x â‰® y)
[â‰°]-to-[â‰®] = contrapositiveáµ£ [<]-to-[â‰¤]

[â‰¥]-to-[>][â‰¡] : âˆ€{a b : â„•} â†’ (a â‰¥ b) â†’ (a > b)âˆ¨(a â‰¡ b)
[â‰¥]-to-[>][â‰¡] {a}{b} (proof) with [â‰¤]-to-[<][â‰¡] {b}{a} (proof)
... | [âˆ¨]-introâ‚—(a<b) = [âˆ¨]-introâ‚—(a<b)
... | [âˆ¨]-introáµ£(bâ‰¡a) = [âˆ¨]-introáµ£(symmetry(_â‰¡_) (bâ‰¡a))

[<]-trichotomy : âˆ€{x y} â†’ (x < y) âˆ¨ (x â‰¡ y) âˆ¨ (x > y)
[<]-trichotomy {x}{y} with converseTotal(_â‰¤_) â¦ƒ [â‰¤]-totality â¦„
[<]-trichotomy {x}{y} | [âˆ¨]-introâ‚— xâ‰¤y with [â‰¤]-to-[<][â‰¡] {x}{y} xâ‰¤y
[<]-trichotomy {x}{y} | [âˆ¨]-introâ‚— xâ‰¤y | [âˆ¨]-introâ‚— x<y = [âˆ¨]-introâ‚— ([âˆ¨]-introâ‚— x<y)
[<]-trichotomy {x}{y} | [âˆ¨]-introâ‚— xâ‰¤y | [âˆ¨]-introáµ£ xâ‰¡y = [âˆ¨]-introâ‚— ([âˆ¨]-introáµ£ xâ‰¡y)
[<]-trichotomy {x}{y} | [âˆ¨]-introáµ£ yâ‰¤x with [â‰¥]-to-[>][â‰¡] {x}{y} yâ‰¤x
[<]-trichotomy {x}{y} | [âˆ¨]-introáµ£ yâ‰¤x | [âˆ¨]-introâ‚— y<x = [âˆ¨]-introáµ£ y<x
[<]-trichotomy {x}{y} | [âˆ¨]-introáµ£ yâ‰¤x | [âˆ¨]-introáµ£ yâ‰¡x = [âˆ¨]-introâ‚— ([âˆ¨]-introáµ£ yâ‰¡x)

[â‰¤][>]-dichotomy : âˆ€{x y} â†’ (x â‰¤ y) âˆ¨ (x > y)
[â‰¤][>]-dichotomy {x}{y} with [<]-trichotomy {x}{y}
[â‰¤][>]-dichotomy {x} {y} | [âˆ¨]-introâ‚— ([âˆ¨]-introâ‚— x<y) = [âˆ¨]-introâ‚—([<]-to-[â‰¤] x<y)
[â‰¤][>]-dichotomy {x} {y} | [âˆ¨]-introâ‚— ([âˆ¨]-introáµ£ xâ‰¡y) = [âˆ¨]-introâ‚—([â‰¡]-to-[â‰¤] xâ‰¡y)
[â‰¤][>]-dichotomy {x} {y} | [âˆ¨]-introáµ£ x>y              = [âˆ¨]-introáµ£(x>y)

[<][â‰¥]-dichotomy : âˆ€{x y} â†’ (x < y) âˆ¨ (x â‰¥ y)
[<][â‰¥]-dichotomy {x}{y} = [âˆ¨]-symmetry([â‰¤][>]-dichotomy {y}{x})

[â‰¯][â‰¢]-to-[â‰±] : âˆ€{a b : â„•} â†’ (a â‰¯ b) â†’ (a â‰¢ b) â†’ (a â‰± b)
[â‰¯][â‰¢]-to-[â‰±] (aâ‰¯b) (aâ‰¢b) (aâ‰¥b) with [â‰¥]-to-[>][â‰¡] (aâ‰¥b)
... | [âˆ¨]-introâ‚— (a>b) = aâ‰¯b a>b
... | [âˆ¨]-introáµ£ (aâ‰¡b) = aâ‰¢b aâ‰¡b

[>][â‰¡]-to-[â‰¥] : âˆ€{a b : â„•} â†’ (a > b)âˆ¨(a â‰¡ b) â†’ (a â‰¥ b)
[>][â‰¡]-to-[â‰¥] {a}{b} ([âˆ¨]-introâ‚—(a<b)) = [<][â‰¡]-to-[â‰¤] {b}{a} ([âˆ¨]-introâ‚—(a<b))
[>][â‰¡]-to-[â‰¥] {a}{b} ([âˆ¨]-introáµ£(bâ‰¡a)) = [<][â‰¡]-to-[â‰¤] {b}{a} ([âˆ¨]-introáµ£(symmetry(_â‰¡_)(bâ‰¡a)))

[>]-to-[â‰¥] : âˆ€{a b : â„•} â†’ (a > b) â†’ (a â‰¥ b)
[>]-to-[â‰¥] {a}{b} (a<b) = [<][â‰¡]-to-[â‰¤] {b}{a} ([âˆ¨]-introâ‚—(a<b))

[â‰±]-to-[â‰¯] : âˆ€{x y : â„•} â†’ (x â‰± y) â†’ (x â‰¯ y)
[â‰±]-to-[â‰¯] = contrapositiveáµ£ [>]-to-[â‰¥]

[â‰®][â‰¯]-to-[â‰¡] : âˆ€{a b : â„•} â†’ (a â‰® b) â†’ (a â‰¯ b) â†’ (a â‰¡ b)
[â‰®][â‰¯]-to-[â‰¡] {a}{b} (aâ‰®b) (aâ‰¯b) with [<]-trichotomy {a}{b}
... | [âˆ¨]-introâ‚— ([âˆ¨]-introâ‚— a<b) = [âŠ¥]-elim(aâ‰®b a<b)
... | [âˆ¨]-introâ‚— ([âˆ¨]-introáµ£ aâ‰¡b) = aâ‰¡b
... | [âˆ¨]-introáµ£ b<a              = [âŠ¥]-elim(aâ‰¯b b<a)

[â‰®][â‰¢][â‰¯]-not : âˆ€{a b : â„•} â†’ (a â‰® b) â†’ (a â‰¢ b) â†’ (a â‰¯ b) â†’ âŠ¥
[â‰®][â‰¢][â‰¯]-not {a}{b} (aâ‰®b) (aâ‰¢b) (aâ‰¯b) with [<]-trichotomy {a}{b}
... | [âˆ¨]-introâ‚— ([âˆ¨]-introâ‚— a<b) = aâ‰®b a<b
... | [âˆ¨]-introâ‚— ([âˆ¨]-introáµ£ aâ‰¡b) = aâ‰¢b aâ‰¡b
... | [âˆ¨]-introáµ£ b<a              = aâ‰¯b b<a

[â‰°][â‰¯]-not : âˆ€{a b : â„•} â†’ (a â‰° b) â†’ (a â‰¯ b) â†’ âŠ¥
[â‰°][â‰¯]-not {a}{b} (aâ‰°b) (aâ‰¯b) = [â‰®][â‰¢][â‰¯]-not ([â‰°]-to-[â‰®] aâ‰°b) ([â‰°]-to-[â‰¢] aâ‰°b) (aâ‰¯b)

[â‰®][â‰±]-not : âˆ€{a b : â„•} â†’ (a â‰® b) â†’ (a â‰± b) â†’ âŠ¥
[â‰®][â‰±]-not {a}{b} (aâ‰®b) (aâ‰±b) = [â‰®][â‰¢][â‰¯]-not (aâ‰®b) ([â‰±]-to-[â‰¢] aâ‰±b) ([â‰±]-to-[â‰¯] aâ‰±b)

[<]-non-zero-existence : âˆ€{a b : â„•} â†’ (a < b) â†’ (ğŸ < b)
[<]-non-zero-existence [â‰¤]-with-[ğ’] = [<]-of-[ğŸ][ğ’]

{-
[+][âˆ’â‚€]-commutativity : âˆ€{x y} â†’ â¦ƒ _ : y â‰¥ z â¦„ â†’ (x + (y âˆ’â‚€ z) â‰¡ (x âˆ’â‚€ z) + y)
-}

[â‰¤]â‚—[+] : âˆ€{x y : â„•} â†’ (x + y â‰¤ x) â†’ (y â‰¡ ğŸ)
[â‰¤]â‚—[+] {ğŸ}               = [â‰¤][0]áµ£
[â‰¤]â‚—[+] {ğ’(x)}{y} (proof) = [â‰¤]â‚—[+] {x} ([â‰¤]-without-[ğ’] {x + y} {x} (proof))

[â‰¤]-with-[+]áµ£ : âˆ€{x y z : â„•} â†’ (x â‰¤ y) â†’ (x + z â‰¤ y + z)
[â‰¤]-with-[+]áµ£ {_}{_}{ğŸ}    (proof)    = proof
[â‰¤]-with-[+]áµ£ {_}{_}{ğ’(z)} (proof) = [â‰¤]-with-[ğ’] â¦ƒ [â‰¤]-with-[+]áµ£ {_}{_}{z} (proof) â¦„

[â‰¤]-with-[+]â‚— : âˆ€{x y z : â„•} â†’ (x â‰¤ y) â†’ (z + x â‰¤ z + y)
[â‰¤]-with-[+]â‚— {.0} {ğŸ}   {z } [â‰¤]-minimum            = reflexivity(_â‰¤_)
[â‰¤]-with-[+]â‚— {.0} {ğ’ y} {z}  [â‰¤]-minimum            = [â‰¤]-successor([â‰¤]-with-[+]â‚— {0}{y}{z} [â‰¤]-minimum)
[â‰¤]-with-[+]â‚— {ğ’ x} {ğ’ y} {z} ([â‰¤]-with-[ğ’] â¦ƒ xy â¦„ ) = [â‰¤]-with-[ğ’] â¦ƒ [â‰¤]-with-[+]â‚— {x} {y} {z} xy â¦„

[â‰¤]-of-[+]áµ£ : âˆ€{x y : â„•} â†’ (y â‰¤ x + y)
[â‰¤]-of-[+]áµ£ {x}   {ğŸ}   = [â‰¤]-minimum
[â‰¤]-of-[+]áµ£ {ğŸ}   {ğ’ x} = reflexivity(_â‰¤_)
[â‰¤]-of-[+]áµ£ {ğ’ x} {ğ’ y} = [â‰¤]-with-[ğ’] â¦ƒ [â‰¤]-of-[+]áµ£ {ğ’ x}{y} â¦„

[â‰¤]-of-[+]â‚— : âˆ€{x y : â„•} â†’ (x â‰¤ x + y)
[â‰¤]-of-[+]â‚— {ğŸ}   {y}   = [â‰¤]-minimum
[â‰¤]-of-[+]â‚— {ğ’ x} {ğŸ}   = reflexivity(_â‰¤_)
[â‰¤]-of-[+]â‚— {ğ’ x} {ğ’ y} =  [â‰¤]-with-[ğ’] â¦ƒ [â‰¤]-of-[+]â‚— {x}{ğ’ y} â¦„

[â‰¤]-with-[+] : âˆ€{xâ‚ yâ‚ : â„•} â†’ â¦ƒ _ : (xâ‚ â‰¤ yâ‚)â¦„ â†’ âˆ€{xâ‚‚ yâ‚‚ : â„•} â†’ â¦ƒ _ : (xâ‚‚ â‰¤ yâ‚‚)â¦„ â†’ (xâ‚ + xâ‚‚ â‰¤ yâ‚ + yâ‚‚)
[â‰¤]-with-[+] {xâ‚} {yâ‚} â¦ƒ x1y1 â¦„ {.0}     {yâ‚‚}     â¦ƒ [â‰¤]-minimum â¦„ = transitivity(_â‰¤_) x1y1 [â‰¤]-of-[+]â‚—
[â‰¤]-with-[+] {xâ‚} {yâ‚} â¦ƒ x1y1 â¦„ {ğ’ xâ‚‚} {ğ’ yâ‚‚} â¦ƒ [â‰¤]-with-[ğ’] â¦ƒ p â¦„ â¦„ = [â‰¤]-with-[ğ’] â¦ƒ [â‰¤]-with-[+] {xâ‚} {yâ‚} {xâ‚‚} {yâ‚‚} â¦„

[â‰¤]-from-[+] : âˆ€{â„“}{P : â„• â†’ Stmt{â„“}}{x} â†’ (âˆ€{n} â†’ P(x + n)) â†’ (âˆ€{y} â†’ â¦ƒ _ : (x â‰¤ y) â¦„ â†’ P(y))
[â‰¤]-from-[+] {â„“} {P} {ğŸ}   anpxn {y}   â¦ƒ [â‰¤]-minimum â¦„        = anpxn{y}
[â‰¤]-from-[+] {â„“} {P} {ğ’ x} anpxn {ğ’ y} â¦ƒ [â‰¤]-with-[ğ’] â¦ƒ xy â¦„ â¦„ = [â‰¤]-from-[+] {â„“} {P âˆ˜ ğ’} {x} anpxn {y} â¦ƒ xy â¦„

[âˆ’â‚€]-move-[ğ’] : âˆ€{x y} â†’ (x â‰¥ y) â†’ ((ğ’(x) âˆ’â‚€ y) â‰¡ ğ’(x âˆ’â‚€ y))
[âˆ’â‚€]-move-[ğ’] {ğŸ}   {ğŸ}    _ = [â‰¡]-intro
[âˆ’â‚€]-move-[ğ’] {ğŸ}   {ğ’(_)} ()
[âˆ’â‚€]-move-[ğ’] {ğ’(_)}{ğŸ}    _ = [â‰¡]-intro
[âˆ’â‚€]-move-[ğ’] {ğ’(x)}{ğ’(y)} ([â‰¤]-with-[ğ’] â¦ƒ proof â¦„) = [âˆ’â‚€]-move-[ğ’] {x}{y} proof
  -- ğ’ğ’x âˆ’â‚€ ğ’y â‰¡ ğ’(ğ’x âˆ’â‚€ ğ’y)
  -- ğ’x âˆ’â‚€ y â‰¡ ğ’(x âˆ’â‚€ y)

[âˆ’â‚€][+]-nullify2 : âˆ€{x y} â†’ (x â‰¤ y) â†” (x + (y âˆ’â‚€ x) â‰¡ y)
[âˆ’â‚€][+]-nullify2 {x}{y} = [â†”]-intro (l{x}{y}) (r{x}{y}) where
  l : âˆ€{x y} â†’ (x â‰¤ y) â† (x + (y âˆ’â‚€ x) â‰¡ y)
  l {ğŸ}   {_}    _     = [â‰¤]-minimum
  l {ğ’(_)}{ğŸ}    ()
  l {ğ’(x)}{ğ’(y)} proof = [â‰¤]-with-[ğ’] â¦ƒ l{x}{y} ([ğ’]-injectivity-raw proof) â¦„

  r : âˆ€{x y} â†’ (x â‰¤ y) â†’ (x + (y âˆ’â‚€ x) â‰¡ y)
  r {ğŸ}   {ğŸ}    proof = [â‰¡]-intro
  r {ğŸ}   {ğ’(_)} proof = [â‰¡]-intro
  r {ğ’(_)}{ğŸ}    ()
  r {ğ’(x)}{ğ’(y)} ([â‰¤]-with-[ğ’] â¦ƒ proof â¦„) = [â‰¡]-with(ğ’) (r{x}{y} (proof))
  -- x + (y âˆ’â‚€ x) â‰¡ y
  -- âˆƒz. x + ((x + z) âˆ’â‚€ x) â‰¡ y
  -- âˆƒz. x + z â‰¡ y
  -- y â‰¡ y

[âˆ’â‚€]-comparison : âˆ€{x y} â†’ (x â‰¤ y) â†” (x âˆ’â‚€ y â‰¡ ğŸ)
[âˆ’â‚€]-comparison {x}{y} = [â†”]-intro (l{x}{y}) (r{x}{y}) where
  l : âˆ€{x y} â†’ (x â‰¤ y) â† (x âˆ’â‚€ y â‰¡ ğŸ)
  l {ğŸ}   {_}    _     = [â‰¤]-minimum
  l {ğ’(_)}{ğŸ}    ()
  l {ğ’(x)}{ğ’(y)} proof = [â‰¤]-with-[ğ’] â¦ƒ l{x}{y} proof â¦„

  r : âˆ€{x y} â†’ (x â‰¤ y) â†’ (x âˆ’â‚€ y â‰¡ ğŸ)
  r {ğŸ}   {_}    proof = [â‰¡]-intro
  r {ğ’(_)}{ğŸ}    ()
  r {ğ’(x)}{ğ’(y)} ([â‰¤]-with-[ğ’] â¦ƒ proof â¦„) = r{x}{y} (proof)

-- TODO: One way to prove this is contraposition of [âˆ’â‚€]-comparison. Another is by [â‰¤]-with-[+]áµ£ and some other stuff, but it seems to require more work
postulate [âˆ’â‚€]-when-non-zero : âˆ€{x y} â†’ (x > y) â†” (x âˆ’â‚€ y > ğŸ)
-- [âˆ’â‚€]-when-non-zero {x}{y} 

[âˆ’â‚€]-lesser-[ğ’]â‚— : âˆ€{x y} â†’ ((x âˆ’â‚€ ğ’(y)) â‰¤ (x âˆ’â‚€ y))
[âˆ’â‚€]-lesser-[ğ’]áµ£ : âˆ€{x y} â†’ ((x âˆ’â‚€ y) â‰¤ (ğ’(x) âˆ’â‚€ y))

[âˆ’â‚€]-lesser-[ğ’]â‚— {ğŸ}   {_}    = [â‰¤]-minimum
[âˆ’â‚€]-lesser-[ğ’]â‚— {ğ’(_)}{ğŸ}    = [â‰¤]-of-[ğ’]
[âˆ’â‚€]-lesser-[ğ’]â‚— {ğ’(x)}{ğ’(y)} = [âˆ’â‚€]-lesser-[ğ’]áµ£ {x}{ğ’(y)}

[âˆ’â‚€]-lesser-[ğ’]áµ£ {ğŸ}   {_}    = [â‰¤]-minimum
[âˆ’â‚€]-lesser-[ğ’]áµ£ {ğ’(x)}{ğŸ}    = [â‰¤]-of-[ğ’]
[âˆ’â‚€]-lesser-[ğ’]áµ£ {ğ’(x)}{ğ’(y)} = [âˆ’â‚€]-lesser-[ğ’]â‚— {ğ’(x)}{y}

[â‰¤][âˆ’â‚€][ğ’]â‚— : âˆ€{x y} â†’ ((ğ’(x) âˆ’â‚€ y) â‰¤ ğ’(x âˆ’â‚€ y))
[â‰¤][âˆ’â‚€][ğ’]â‚— {x}   {ğŸ}    = reflexivity(_â‰¤_)
[â‰¤][âˆ’â‚€][ğ’]â‚— {ğŸ}   {ğ’(y)} = [â‰¤]-minimum
[â‰¤][âˆ’â‚€][ğ’]â‚— {ğ’(x)}{ğ’(y)} = [â‰¤][âˆ’â‚€][ğ’]â‚— {x}{y}

[âˆ’â‚€]-lesser : âˆ€{x y} â†’ ((x âˆ’â‚€ y) â‰¤ x)
[âˆ’â‚€]-lesser {ğŸ}   {_}    = [â‰¤]-minimum
[âˆ’â‚€]-lesser {ğ’(x)}{ğŸ}    = reflexivity(_â‰¤_)
[âˆ’â‚€]-lesser {ğ’(x)}{ğ’(y)} = ([âˆ’â‚€]-lesser-[ğ’]â‚— {ğ’(x)}{y}) ğŸ– ([âˆ’â‚€]-lesser {ğ’(x)}{y})

[âˆ’â‚€]-positive : âˆ€{x y} â†’ (y > x) â†’ (y âˆ’â‚€ x > 0) -- TODO: Converse is probably also true
[âˆ’â‚€]-positive {ğŸ}   {ğŸ}    ()
[âˆ’â‚€]-positive {ğ’(x)}{ğŸ}    ()
[âˆ’â‚€]-positive {ğŸ}   {ğ’(y)} (_) = [â‰¤]-with-[ğ’] â¦ƒ [â‰¤]-minimum â¦„
[âˆ’â‚€]-positive {ğ’(x)}{ğ’(y)} ([â‰¤]-with-[ğ’] â¦ƒ proof â¦„) = [âˆ’â‚€]-positive {x}{y} (proof)
  -- (ğ’y > ğ’x) â†’ (ğ’y âˆ’â‚€ ğ’x > 0)
  -- (ğ’x < ğ’y) â†’ (0 < ğ’y âˆ’â‚€ ğ’x)
  -- (ğ’ğ’x â‰¤ ğ’y) â†’ (ğ’0 â‰¤ ğ’y âˆ’â‚€ ğ’x)
  -- (ğ’x â‰¤ y) â†’ (ğ’0 â‰¤ ğ’y âˆ’â‚€ ğ’x)
  -- (ğ’x â‰¤ y) â†’ (ğ’0 â‰¤ y âˆ’â‚€ x)
  -- (x < y) â†’ (0 < y âˆ’â‚€ x)
  -- (y > x) â†’ (y âˆ’â‚€ x > 0)

[âˆ’â‚€]-nested-sameâ‚— : âˆ€{x y} â†’ (x â‰¥ y) â†” (x âˆ’â‚€ (x âˆ’â‚€ y) â‰¡ y)
[âˆ’â‚€]-nested-sameâ‚— {x}{y} = [â†”]-intro (l{x}{y}) (r{x}{y}) where
  l : âˆ€{x y} â†’ (x â‰¥ y) â† (x âˆ’â‚€ (x âˆ’â‚€ y) â‰¡ y)
  l {x}{y} proof =
    [â‰¡]-to-[â‰¤] (symmetry(_â‰¡_) proof)
    ğŸ– [âˆ’â‚€]-lesser {x}{x âˆ’â‚€ y}

  r : âˆ€{x y} â†’ (x â‰¥ y) â†’ (x âˆ’â‚€ (x âˆ’â‚€ y) â‰¡ y)
  r{x}{y} xâ‰¥y =
    [â‰¡]-with(_âˆ’â‚€ (x âˆ’â‚€ y)) (symmetry(_â‰¡_) ([â†”]-to-[â†’] ([âˆ’â‚€][+]-nullify2 {y}{x}) (xâ‰¥y)) ğŸ– [+]-commutativity-raw{y}{x âˆ’â‚€ y})
    ğŸ– [âˆ’â‚€]â‚—[+]â‚—-nullify {x âˆ’â‚€ y}{y}
      -- x âˆ’â‚€ (x âˆ’â‚€ y)
      -- ((x âˆ’â‚€ y) + y) âˆ’â‚€ (x âˆ’â‚€ y)
      -- y

[ğ„©]-of-ğ’â‚— : âˆ€{x y} â†’ (x â‰¥ y) â†’ (ğ’(x) ğ„© y â‰¡ ğ’(x ğ„© y))
[ğ„©]-of-ğ’â‚— {ğŸ}   {ğŸ}   xy = [â‰¡]-intro
[ğ„©]-of-ğ’â‚— {ğ’ x} {ğŸ}   xy = [â‰¡]-intro
[ğ„©]-of-ğ’â‚— {ğ’ x} {ğ’ y} xy = [ğ„©]-of-ğ’â‚— {x} {y} ([â‰¤]-without-[ğ’] xy)

[ğ„©]-of-ğ’áµ£ : âˆ€{x y} â†’ (x â‰¤ y) â†’ (x ğ„© ğ’(y) â‰¡ ğ’(x ğ„© y))
[ğ„©]-of-ğ’áµ£ {ğŸ}   {ğŸ}   xy = [â‰¡]-intro
[ğ„©]-of-ğ’áµ£ {ğŸ}   {ğ’ y} xy = [â‰¡]-intro
[ğ„©]-of-ğ’áµ£ {ğ’ x} {ğ’ y} xy = [ğ„©]-of-ğ’áµ£ {x} {y} ([â‰¤]-without-[ğ’] xy)
