module Numeral.Integer.Oper where

open import Numeral.Natural      as â„• using (â„•)
import      Numeral.Natural.Oper as â„•
open import Numeral.Integer
open import Numeral.Integer.Sign
import      Numeral.Sign       as Sign
import      Numeral.Sign.Oper0 as Sign

-- Unclosed total subtraction from natural numbers to integers
_âˆ’â‚™_ : â„• â†’ â„• â†’ â„¤
x      âˆ’â‚™ â„•.ğŸ    = â„¤.+â‚™ x
â„•.ğŸ    âˆ’â‚™ â„•.ğ’(x) = â„¤.âˆ’ğ’â‚™(x)
â„•.ğ’(x) âˆ’â‚™ â„•.ğ’(y) = x âˆ’â‚™ y

-- Construction of an integer with the sign and numeral components
signed : (Sign.+|âˆ’) â†’ â„• â†’ â„¤
signed (Sign.â•) (n) = +â‚™ n
signed (Sign.â–) (n) = âˆ’â‚™ n

signed0 : (Sign.+|0|âˆ’) â†’ â„• â†’ â„¤
signed0(Sign.â•) (â„•.ğ’(n)) = +ğ’â‚™(n)
signed0(Sign.â–) (â„•.ğ’(n)) = âˆ’ğ’â‚™(n)
{-# CATCHALL #-}
signed0(_)      (_)      = ğŸ

------------------------------------------
-- Unary operations

-- Predecessor
ğ : â„¤ â†’ â„¤
ğ(+ğ’â‚™(n)) = +â‚™ n
ğ(ğŸ)      = âˆ’ğ’â‚™(â„•.ğŸ)
ğ(âˆ’ğ’â‚™(n)) = âˆ’ğ’â‚™(â„•.ğ’(n))

-- Successor
ğ’ : â„¤ â†’ â„¤
ğ’(+â‚™ n)        = +â‚™ â„•.ğ’(n)
ğ’(âˆ’ğ’â‚™(â„•.ğŸ))    = +â‚™ â„•.ğŸ
ğ’(âˆ’ğ’â‚™(â„•.ğ’(n))) = âˆ’ğ’â‚™(n)

-- Identity
+_ : â„¤ â†’ â„¤
+ n = n

-- Negation
âˆ’_ : â„¤ â†’ â„¤
âˆ’ ğŸ = ğŸ
âˆ’ (+ğ’â‚™(n)) = âˆ’ğ’â‚™(n)
âˆ’ (âˆ’ğ’â‚™(n)) = +ğ’â‚™(n)

-- Absolute value
abs : â„¤ â†’ â„¤
abs(+â‚™ x)  = +â‚™ x
abs(âˆ’ğ’â‚™ x) = +ğ’â‚™ x

------------------------------------------
-- Binary operations

infixl 10010 _+_
infixl 10020 _â‹…_

-- Addition
_+_ : â„¤ â†’ â„¤ â†’ â„¤
(+â‚™  x) + (+â‚™  y) = +â‚™ (x â„•.+ y)
(âˆ’ğ’â‚™ x) + (âˆ’ğ’â‚™ y) = âˆ’ğ’â‚™(â„•.ğ’(x â„•.+ y))
(+â‚™  x) + (âˆ’ğ’â‚™ y) = x âˆ’â‚™ â„•.ğ’(y)
(âˆ’ğ’â‚™ x) + (+â‚™  y) = (+â‚™ y) + (âˆ’ğ’â‚™ x)

-- Subtraction
_âˆ’_ : â„¤ â†’ â„¤ â†’ â„¤
x âˆ’ y = x + (âˆ’ y)

-- Multiplication
_â‹…_ : â„¤ â†’ â„¤ â†’ â„¤
x â‹… y = signed0 ((sign0 x) Sign.â¨¯ (sign0 y)) ((absâ‚™ x) â„•.â‹… (absâ‚™ y))

-- Distance
_ğ„©_ : â„¤ â†’ â„¤ â†’ â„•
(+â‚™  x)     ğ„© (+â‚™  y)     = x â„•.ğ„© y
(âˆ’ğ’â‚™ x)     ğ„© (âˆ’ğ’â‚™ y)     = x â„•.ğ„© y
(+â‚™(â„•.ğŸ))   ğ„© (âˆ’ğ’â‚™ y)     = â„•.ğ’(y)
(+â‚™(â„•.ğ’ x)) ğ„© (âˆ’ğ’â‚™ y)     = â„•.ğ’((+â‚™ x) ğ„© (âˆ’ğ’â‚™ y))
(âˆ’ğ’â‚™ x)     ğ„© (+â‚™(â„•.ğŸ))   = â„•.ğ’(x)
(âˆ’ğ’â‚™ x)     ğ„© (+â‚™(â„•.ğ’ y)) = â„•.ğ’((âˆ’ğ’â‚™ x) ğ„© (+â‚™ y))
