module Sets.IterativeSet where

import      Lvl
open import Data
open import Data.Boolean
open import Data.Boolean.Stmt
open import Data.Either as Either using (_â€–_)
open import Data.Tuple as Tuple using ()
open import Functional
open import Logic
open import Logic.Propositional
open import Logic.Predicate
open import Relator.Equals using () renaming (_â‰¡_ to Id ; [â‰¡]-intro to intro)
open import Syntax.Function
open import Type
open import Type.Dependent

module _ where
  private variable {â„“â‚ â„“â‚‚} : Lvl.Level

  -- A model of constructive set theory (CZF) using iterative sets. (TODO: Not sure. Filter does not work?)
  record Iset : Type{Lvl.ğ’(â„“â‚)} where
    coinductive
    constructor intro
    field
      {Index} : Type{â„“â‚}
      elem : Index â†’ Iset{â„“â‚}
  open Iset

{- TODO: Neither provable or unprovable?
  Iset-no-eta-identity1 : âˆ€{A : Iset{â„“â‚}} â†’ Â¬(Id A (intro(elem A)))
  Iset-no-eta-identity1 {A = _} ()

  Iset-no-eta-identity2 : âˆ€{I : Type{â„“â‚}}{e : I â†’ Iset{â„“â‚}} â†’ Â¬(Id (Iset.intro{Index = I}(e)) (Iset.intro{Index = I}(e)))
  Iset-no-eta-identity2 ()
-}

  âˆ… : Iset{â„“â‚}
  âˆ… = intro{Index = Empty} empty

  singleton : Iset{â„“â‚} â†’ Iset{â„“â‚}
  singleton = intro{Index = Unit} âˆ˜ const

  pair : Iset{â„“â‚} â†’ Iset{â„“â‚} â†’ Iset{â„“â‚}
  pair A B = intro{Index = Lvl.Up(Bool)} \{(Lvl.up ğ¹) â†’ A ; (Lvl.up ğ‘‡) â†’ B}

  _âˆª_ : Iset{â„“â‚} â†’ Iset{â„“â‚} â†’ Iset{â„“â‚}
  A âˆª B = intro{Index = Index(A) â€– Index(B)} (Either.map1 (elem(A)) (elem(B)))

  _,_ : Iset{â„“â‚} â†’ Iset{â„“â‚} â†’ Iset{â„“â‚}
  A , B = pair (singleton A) (pair A B)

  _â¨¯_ : Iset{â„“â‚} â†’ Iset{â„“â‚} â†’ Iset{â„“â‚}
  A â¨¯ B = intro{Index = Index(A) Tuple.â¨¯ Index(B)} \{(ia Tuple., ib) â†’ (elem(A)(ia) , elem(B)(ib))}

  â‹ƒ : Iset{â„“â‚} â†’ Iset{â„“â‚}
  â‹ƒ A = intro{Index = Î£(Index(A)) (ia â†¦ Index(elem(A)(ia)))} (\{(intro ia i) â†’ elem(elem(A)(ia))(i)})

  filter : (A : Iset{â„“â‚}) â†’ (Index(A) â†’ Stmt{â„“â‚}) â†’ Iset{â„“â‚}
  filter A P = intro {Index = Î£(Index(A)) P} (elem(A) âˆ˜ Î£.left)

  {-
  filter2 : (A : Iset{Lvl.ğ’ â„“â‚}) â†’ (Iset{â„“â‚} â†’ Stmt{â„“â‚}) â†’ Iset{Lvl.ğ’ â„“â‚}
  filter2 A P = intro {Index = Î£(Iset) P} (\{(intro i p) â†’ {!i!}})
  -- intro i p
  -}

  filterBool : (A : Iset{â„“â‚}) â†’ (Index(A) â†’ Bool) â†’ Iset{â„“â‚}
  filterBool A f = filter A (Lvl.Up âˆ˜ IsTrue âˆ˜ f)

  â„˜ : Iset{â„“â‚} â†’ Iset{â„“â‚}
  â„˜ A = intro{Index = Index(A) â†’ Bool} (filterBool A)
  -- intro{Index = Index(A) â†’ Stmt} (filter A)
  -- TODO: How should one use Stmt and filter instead? The levels become a problem

  record _â‰¡_ (A : Iset{â„“â‚}) (B : Iset{â„“â‚}) : Type{â„“â‚}
  record _âŠ†_ (A : Iset{â„“â‚}) (B : Iset{â„“â‚}) : Type{â„“â‚}
  _âŠ‡_ : Iset{â„“â‚} â†’ Iset{â„“â‚} â†’ Type{â„“â‚}

  record _â‰¡_ A B where
    coinductive
    constructor intro
    field
      left  : A âŠ‡ B
      right : A âŠ† B

  _âˆˆ_ : Iset{â„“â‚} â†’ Iset{â„“â‚} â†’ Type{â„“â‚}
  a âˆˆ B = âˆƒ{Obj = Index(B)} (ib â†¦ a â‰¡ elem(B)(ib))

  record _âŠ†_ A B where
    inductive
    constructor intro
    field
      map : Index(A) â†’ Index(B)
      proof : âˆ€{ia} â†’ (elem(A)(ia) â‰¡ elem(B)(map(ia)))

  A âŠ‡ B = B âŠ† A
  module _âŠ‡_ where
    open _âŠ†_ public

  _âˆ‰_ : Iset{â„“â‚} â†’ Iset{â„“â‚} â†’ Type{â„“â‚}
  a âˆ‰ B = Â¬(a âˆˆ B)

  [â‰¡]-to-[âŠ†] : âˆ€{A B : Iset{â„“â‚}} â†’ (A â‰¡ B) â†’ (A âŠ† B)
  [â‰¡]-to-[âŠ†] = _â‰¡_.right

  [â‰¡]-to-[âŠ‡] : âˆ€{A B : Iset{â„“â‚}} â†’ (A â‰¡ B) â†’ (A âŠ‡ B)
  [â‰¡]-to-[âŠ‡] = _â‰¡_.left

  [â‰¡]-reflexivity : âˆ€{A : Iset{â„“â‚}} â†’ (A â‰¡ A)
  [âŠ†]-reflexivity : âˆ€{A : Iset{â„“â‚}} â†’ (A âŠ† A)
  [âŠ‡]-reflexivity : âˆ€{A : Iset{â„“â‚}} â†’ (A âŠ‡ A)

  _â‰¡_.left ([â‰¡]-reflexivity {A = A}) = [âŠ‡]-reflexivity {A = A}
  _â‰¡_.right ([â‰¡]-reflexivity {A = A}) = [âŠ†]-reflexivity {A = A}

  _âŠ†_.map    [âŠ†]-reflexivity = id
  _âŠ†_.proof ([âŠ†]-reflexivity {A = A}) {i} = [â‰¡]-reflexivity {A = elem(A)(i)}

  [âŠ‡]-reflexivity = [âŠ†]-reflexivity

  [â‰¡]-symmetry : âˆ€{A B : Iset{â„“â‚}} â†’ (A â‰¡ B) â†’ (B â‰¡ A)
  _â‰¡_.left  ([â‰¡]-symmetry {A = A}{B = B} ab) = _â‰¡_.right ab
  _â‰¡_.right ([â‰¡]-symmetry {A = A}{B = B} ab) = _â‰¡_.left ab

  [â‰¡]-transitivity : âˆ€{A B C : Iset{â„“â‚}} â†’ (A â‰¡ B) â†’ (B â‰¡ C) â†’ (A â‰¡ C)
  [âŠ†]-transitivity : âˆ€{A B C : Iset{â„“â‚}} â†’ (A âŠ† B) â†’ (B âŠ† C) â†’ (A âŠ† C)
  [âŠ‡]-transitivity : âˆ€{A B C : Iset{â„“â‚}} â†’ (A âŠ‡ B) â†’ (B âŠ‡ C) â†’ (A âŠ‡ C)

  _â‰¡_.left  ([â‰¡]-transitivity {A = A}{B = B}{C = C} ab bc) = [âŠ‡]-transitivity {A = A}{B = B}{C = C} (_â‰¡_.left ab) (_â‰¡_.left bc)
  _â‰¡_.right ([â‰¡]-transitivity {A = A}{B = B}{C = C} ab bc) = [âŠ†]-transitivity {A = A}{B = B}{C = C} (_â‰¡_.right ab) (_â‰¡_.right bc)

  _âŠ†_.map   ([âŠ†]-transitivity {A = A} {B = B} {C = C} ab bc) = _âŠ†_.map bc âˆ˜ _âŠ†_.map ab
  _âŠ†_.proof ([âŠ†]-transitivity {A = A} {B = B} {C = C} ab bc) {ia} = [â‰¡]-transitivity {A = elem(A)(ia)}{B = elem B (_âŠ†_.map ab ia)} {C = elem(C)((_âŠ†_.map bc)((_âŠ†_.map ab)(ia)))} (_âŠ†_.proof ab {ia}) (_âŠ†_.proof bc)

  [âŠ‡]-transitivity {A = A} {B = B} {C = C} ab bc = [âŠ†]-transitivity {A = C}{B = B}{C = A} bc ab

  [âŠ†]-antisymmetry : âˆ€{A B : Iset{â„“â‚}} â†’ (A âŠ‡ B) â†’ (A âŠ† B) â†’ (A â‰¡ B)
  [âŠ†]-antisymmetry = intro

  [âŠ‡]-antisymmetry : âˆ€{A B : Iset{â„“â‚}} â†’ (A âŠ† B) â†’ (A âŠ‡ B) â†’ (A â‰¡ B)
  [âŠ‡]-antisymmetry = swap intro

  [âˆˆ]-of-elem : âˆ€{A : Iset{â„“â‚}}{ia : Index(A)} â†’ (elem(A)(ia) âˆˆ A)
  âˆƒ.witness ([âˆˆ]-of-elem {ia = ia}) = ia
  âˆƒ.proof    [âˆˆ]-of-elem = [â‰¡]-reflexivity

  Iset-intro-self-equality : âˆ€{A : Iset{â„“â‚}} â†’ (intro{Index = Index(A)}(elem(A)) â‰¡ A)
  _âŠ†_.map   (_â‰¡_.left  Iset-intro-self-equality) = id
  _âŠ†_.map   (_â‰¡_.right Iset-intro-self-equality) = id
  _âŠ†_.proof (_â‰¡_.left  Iset-intro-self-equality) = [â‰¡]-reflexivity
  _âŠ†_.proof (_â‰¡_.right Iset-intro-self-equality) = [â‰¡]-reflexivity

  [âŠ†]-with-elem : âˆ€{x y : Iset{â„“â‚}} â†’ (xy : x âŠ† y) â†’ âˆ€{ix} â†’ (elem x ix â‰¡ elem y (_âŠ†_.map xy ix))
  [âŠ†]-with-elem (intro map proof) {ix} = proof{ix}

  [âŠ†]-inclusion : âˆ€{A : Iset{â„“â‚}}{B : Iset{â„“â‚}} â†’ (âˆ€{x : Iset{â„“â‚}} â†’ (x âˆˆ A) â†’ (x âˆˆ B)) â†” (A âŠ† B)
  [âŠ†]-inclusion {A = A}{B = B} = [â†”]-intro l r where
    l : (âˆ€{x} â†’ (x âˆˆ A) â†’ (x âˆˆ B)) â† (A âŠ† B)
    âˆƒ.witness (l (intro map proof) {x} xa) = map(âˆƒ.witness xa)
    âˆƒ.proof   (l (intro map proof) {x} xa) = [â‰¡]-transitivity (âˆƒ.proof xa) proof

    r : (âˆ€{x} â†’ (x âˆˆ A) â†’ (x âˆˆ B)) â†’ (A âŠ† B)
    _âŠ†_.map   (r proof) ia = [âˆƒ]-witness (proof{x = elem(A)(ia)} ([âˆˆ]-of-elem {A = A}))
    _âŠ†_.proof (r proof) {ia} = [âˆƒ]-proof (proof([âˆˆ]-of-elem {A = A}))

  [âŠ‡]-inclusion : âˆ€{A : Iset{â„“â‚}}{B : Iset{â„“â‚}} â†’ (âˆ€{x : Iset{â„“â‚}} â†’ (x âˆˆ A) â† (x âˆˆ B)) â†” (A âŠ‡ B)
  [âŠ‡]-inclusion {A = A}{B = B} = [âŠ†]-inclusion {A = B}{B = A}

  [â‰¡]-inclusion : âˆ€{A : Iset{â„“â‚}}{B : Iset{â„“â‚}} â†’ (âˆ€{x : Iset{â„“â‚}} â†’ (x âˆˆ A) â†” (x âˆˆ B)) â†” (A â‰¡ B)
  Tuple.left  (Tuple.left ([â‰¡]-inclusion {A = A} {B = B}) ab) = [â†”]-to-[â†] [âŠ‡]-inclusion (_â‰¡_.left ab)
  Tuple.right (Tuple.left ([â‰¡]-inclusion {A = A} {B = B}) ab) = [â†”]-to-[â†] [âŠ†]-inclusion (_â‰¡_.right ab)
  _â‰¡_.left  (Tuple.right ([â‰¡]-inclusion {A = A} {B = B}) xaxb) = [â†”]-to-[â†’] [âŠ‡]-inclusion ([â†”]-to-[â†] xaxb)
  _â‰¡_.right (Tuple.right ([â‰¡]-inclusion {A = A} {B = B}) xaxb) = [â†”]-to-[â†’] [âŠ†]-inclusion ([â†”]-to-[â†’] xaxb)

  âˆ…-inclusion : âˆ€{x : Iset{â„“â‚}} â†’ (x âˆ‰ âˆ…)
  âˆ…-inclusion ()

  singleton-inclusion : âˆ€{a x : Iset{â„“â‚}} â†’ (x âˆˆ singleton(a)) â†” (x â‰¡ a)
  Tuple.left (singleton-inclusion {a = a} {x}) xin = [âˆƒ]-intro <> â¦ƒ xin â¦„
  Tuple.right (singleton-inclusion {a = a} {x}) ([âˆƒ]-intro i â¦ƒ eq â¦„ ) = eq

  [âˆª]-inclusion : âˆ€{A B x : Iset{â„“â‚}} â†’ (x âˆˆ (A âˆª B)) â†” (x âˆˆ A)âˆ¨(x âˆˆ B)
  Tuple.left ([âˆª]-inclusion {A = A} {B} {x}) ([âˆ¨]-introâ‚— ([âˆƒ]-intro ia)) = [âˆƒ]-intro (Either.Left  ia)
  Tuple.left ([âˆª]-inclusion {A = A} {B} {x}) ([âˆ¨]-introáµ£ ([âˆƒ]-intro ib)) = [âˆƒ]-intro (Either.Right ib)
  Tuple.right ([âˆª]-inclusion {A = A} {B} {x}) ([âˆƒ]-intro ([âˆ¨]-introâ‚— ia)) = [âˆ¨]-introâ‚— ([âˆƒ]-intro ia)
  Tuple.right ([âˆª]-inclusion {A = A} {B} {x}) ([âˆƒ]-intro ([âˆ¨]-introáµ£ ib)) = [âˆ¨]-introáµ£ ([âˆƒ]-intro ib)

  [â‹ƒ]-inclusion : âˆ€{A x : Iset{â„“â‚}} â†’ (x âˆˆ (â‹ƒ A)) â†” âˆƒ(a â†¦ (a âˆˆ A) âˆ§ (x âˆˆ a))
  Î£.left  (âˆƒ.witness (Tuple.left ([â‹ƒ]-inclusion {A = A} {x}) ([âˆƒ]-intro a â¦ƒ [âˆ§]-intro ([âˆƒ]-intro iA) _ â¦„))) = iA
  Î£.right (âˆƒ.witness (Tuple.left ([â‹ƒ]-inclusion {A = A} {x}) ([âˆƒ]-intro a â¦ƒ [âˆ§]-intro ([âˆƒ]-intro iA â¦ƒ aA â¦„) ([âˆƒ]-intro ia) â¦„))) = _âŠ†_.map (_â‰¡_.right aA) ia
  âˆƒ.proof (Tuple.left ([â‹ƒ]-inclusion {A = A} {x}) ([âˆƒ]-intro a â¦ƒ [âˆ§]-intro ([âˆƒ]-intro iA â¦ƒ aA â¦„) ([âˆƒ]-intro ia â¦ƒ xa â¦„) â¦„)) = [â‰¡]-transitivity xa ([âŠ†]-with-elem ([â‰¡]-to-[âŠ†] aA) {ia})
  âˆƒ.witness (Tuple.right ([â‹ƒ]-inclusion {A = A} {x}) ([âˆƒ]-intro (intro iA ia) â¦ƒ proof â¦„)) = elem(A)(iA)
  Tuple.left (âˆƒ.proof (Tuple.right ([â‹ƒ]-inclusion {A = A} {x}) ([âˆƒ]-intro (intro iA ia) â¦ƒ proof â¦„))) = [âˆˆ]-of-elem {A = A}
  âˆƒ.witness (Tuple.right (âˆƒ.proof (Tuple.right ([â‹ƒ]-inclusion {A = A} {x}) ([âˆƒ]-intro (intro iA ia) â¦ƒ proof â¦„)))) = ia
  âˆƒ.proof (Tuple.right (âˆƒ.proof (Tuple.right ([â‹ƒ]-inclusion {A = A} {x}) ([âˆƒ]-intro (intro iA ia) â¦ƒ proof â¦„)))) = proof

  {-
  filter-inclusion : âˆ€{A : Iset{â„“â‚}}{i : Index(A)}{P} â†’ (elem(A)(i) âˆˆ filter A P) â†” P(i)
  Î£.left             (âˆƒ.witness (Tuple.left (filter-inclusion {i = i}) pi)) = i
  Î£.right            (âˆƒ.witness (Tuple.left (filter-inclusion {i = i}) pi)) = pi
  _â‰¡_.left  (âˆƒ.proof (Tuple.left filter-inclusion pi)) = intro id [â‰¡]-reflexivity
  _â‰¡_.right (âˆƒ.proof (Tuple.left filter-inclusion pi)) = intro id [â‰¡]-reflexivity
  Tuple.right (filter-inclusion {i = i}) ([âˆƒ]-intro (intro iA PiA) â¦ƒ [â‰¡]-intro â¦„) = {!!}
  -- {!_âŠ‡_.proof ([â‰¡]-to-[âŠ‡] proof) {intro ? ?}!}
  -}

  -- Iset-induction : âˆ€{P : Iset{â„“â‚} â†’ Stmt{â„“â‚‚}} â†’ (âˆ€{I : Type{â„“â‚}}{e : I â†’ Iset{â„“â‚}} â†’ ((âˆ€{i : I} â†’ P(e(i))) â†’ P(Iset.intro(e)))) â†’ (âˆ€{A : Iset{â„“â‚}} â†’ P(A))
  -- Iset-induction {P = P} proof {A} = proof {Index(A)} {elem(A)} ?

  --Iset-induction : âˆ€{P : Iset{â„“â‚} â†’ Stmt{â„“â‚‚}} â†’ (âˆ€{A : Iset{â„“â‚}} â†’ (âˆ€{i : Index(A)} â†’ P(elem(A)(i))) â†’ P(A)) â†’ (âˆ€{A : Iset{â„“â‚}} â†’ P(A))
  -- Iset-induction {â„“â‚} {â„“â‚‚} {P} proof {A} = proof{A} \{i} â†’ Iset-induction{P = P} proof {elem(A)(i)}

  -- Iset-2-2 : âˆ€{P : Iset{â„“â‚} â†’ Stmt{â„“â‚‚}} â†’ (âˆ€{x : Iset{â„“â‚}} â†’ (âˆ€{y : Iset{â„“â‚}} â†’ (y âˆˆ x) â†’ P(y) â†’ P(x))) â†’ (âˆ€{A : Iset{â„“â‚}} â†’ P(A))
  -- Iset-2-2 {P = P} proof {A = A} = Iset-induction {P = P} {Index(A)}{elem(A)} (p â†¦ proof {intro (elem(A))}{A} {!!} {!!}) {A = A}
