{-# OPTIONS --cubical #-}

module Miscellaneous.LimNatural where

import      Lvl
open import Numeral.Natural as â„• using (â„•)
open import Numeral.Sign as Sign using (âˆ’|+ ; âˆ’|0|+ ; â– ; â•)
open import Type.Cubical
open import Type.Cubical.Path.Equality
open import Type

data â„•âˆ : Type{Lvl.ğŸ} where
  ğŸ : â„•âˆ
  ğ’ : â„•âˆ â†’ â„•âˆ
  âˆ : â„•âˆ
  ğ’-fixpoint : (ğ’(âˆ) â‰¡ âˆ)

ğâ‚€ : â„•âˆ â†’ â„•âˆ
ğâ‚€(ğŸ)    = ğŸ
ğâ‚€(ğ’(n)) = n
ğâ‚€(âˆ)    = âˆ
ğâ‚€(ğ’-fixpoint i) = âˆ

_+_ : â„•âˆ â†’ â„•âˆ â†’ â„•âˆ
x + ğŸ    = x
x + ğ’(y) = ğ’(x + y)
_ + âˆ    = âˆ
x + ğ’-fixpoint i = ğ’-fixpoint i
infixl 10010 _+_

_â‹…_ : â„•âˆ â†’ â„•âˆ â†’ â„•âˆ
x â‹… ğŸ    = ğŸ
x â‹… ğ’(y) = x + (x â‹… y)
x â‹… âˆ    = âˆ
x â‹… ğ’-fixpoint i = âˆ
infixl 10020 _â‹…_

open import Data.Boolean
open import Data.Boolean.Stmt
open import Functional
open import Type.Cubical.Path.Proofs

isFinite : â„•âˆ â†’ Bool
isFinite ğŸ      = ğ‘‡
isFinite (ğ’(n)) = isFinite n
isFinite âˆ      = ğ¹
isFinite (ğ’-fixpoint i) = ğ¹

isZero : â„•âˆ â†’ Bool
isZero ğŸ     = ğ‘‡
isZero (ğ’ _) = ğ¹
isZero âˆ     = ğ¹
isZero (ğ’-fixpoint i) = ğ¹

_â‰¤?_ : â„•âˆ â†’ â„•âˆ â†’ Bool
ğŸ    â‰¤? _    = ğ‘‡
ğ’(x) â‰¤? ğŸ    = ğ¹
ğ’(x) â‰¤? ğ’(y) = x â‰¤? y
ğ’(x) â‰¤? âˆ    = ğ‘‡
âˆ    â‰¤? ğŸ    = ğ¹
âˆ    â‰¤? ğ’(y) = âˆ â‰¤? y
âˆ    â‰¤? âˆ    = ğ‘‡
ğ’(ğŸ)            â‰¤? ğ’-fixpoint _ = ğ‘‡
ğ’(ğ’(x))         â‰¤? ğ’-fixpoint _ = ğ‘‡
ğ’(âˆ)            â‰¤? ğ’-fixpoint _ = ğ‘‡
ğ’(ğ’-fixpoint _) â‰¤? ğ’-fixpoint _ = ğ‘‡
âˆ               â‰¤? ğ’-fixpoint _ = ğ‘‡
ğ’-fixpoint _    â‰¤? ğŸ            = ğ¹
ğ’-fixpoint _    â‰¤? ğ’(y)         = âˆ â‰¤? y
ğ’-fixpoint _    â‰¤? âˆ            = ğ‘‡
ğ’-fixpoint _    â‰¤? ğ’-fixpoint _ = ğ‘‡

_â‰¤_ : â„•âˆ â†’ â„•âˆ â†’ Type
_â‰¤_ = IsTrue âˆ˜â‚‚ (_â‰¤?_)

open import Data
open import Structure.Function.Domain
open import Structure.Function
open import Structure.Relator.Properties
import      Structure.Relator.Names as Names
open import Syntax.Transitivity
open import Type.Cubical.Path.Proofs

private variable x y z : â„•âˆ

ğ’-âˆ-involutive : (ğ’(ğ’(âˆ)) â‰¡ âˆ)
ğ’-âˆ-involutive = congruenceâ‚(ğ’) ğ’-fixpoint ğŸ– ğ’-fixpoint

instance
  ğ’-injectivity : Injective(ğ’)
  Injective.proof ğ’-injectivity = congruenceâ‚(ğâ‚€)

[+]-baseâ‚— : (ğŸ + x â‰¡ x)
[+]-baseâ‚— {ğŸ}   = reflexivity(_â‰¡_)
[+]-baseâ‚— {ğ’ x} = congruenceâ‚(ğ’) ([+]-baseâ‚— {x})
[+]-baseâ‚— {âˆ}   = reflexivity(_â‰¡_)
[+]-baseâ‚— {ğ’-fixpoint i} = reflexivity(_â‰¡_) {ğ’-fixpoint i}

[+]-stepâ‚— : (ğ’(x) + y â‰¡ ğ’(x + y))
[+]-stepâ‚— {x} {ğŸ}   = reflexivity(_â‰¡_)
[+]-stepâ‚— {x} {ğ’ y} = congruenceâ‚(ğ’) ([+]-stepâ‚— {x}{y})
[+]-stepâ‚— {x} {âˆ}   = symmetry(_â‰¡_) ğ’-fixpoint
[+]-stepâ‚— {x} {ğ’-fixpoint i} = symmetry(_â‰¡_) (Interval.hComp diagram {!ğ’-fixpoint-fixpoint i!}) where
  diagram : Interval â†’ Interval.Partial(Interval.farBound i) _
  diagram _ (i = Interval.ğŸ) = congruenceâ‚(ğ’) ğ’-fixpoint
  diagram _ (i = Interval.ğŸ) = ğ’-fixpoint
  
  {-
  i0 j0 ğ’âˆ
  i0 j1 ğ’ğ’âˆ
  i1 j0 âˆ
  i1 j1 ğ’âˆ
  -}
  -- test : âˆ€{i} â†’ (ğ’(ğ’-fixpoint i) â‰¡ ğ’-fixpoint i)
  -- test {i} j = {!!}
  {-
  i0 j0 ğ’ğ’âˆ
  i0 j1 ğ’âˆ
  i1 j0 ğ’âˆ
  i1 j1 âˆ
  -}

open import Structure.Operator.Properties
import      Structure.Operator.Names as Names

instance
  [+]-identityáµ£ : Identityáµ£(_+_)(ğŸ)
  Identityáµ£.proof [+]-identityáµ£ = reflexivity(_â‰¡_)

instance
  [+]-identityâ‚— : Identityâ‚—(_+_)(ğŸ)
  [+]-identityâ‚— = intro proof where
    proof : Names.Identityâ‚—(_+_)(ğŸ)
    proof {ğŸ}   = reflexivity(_â‰¡_)
    proof {ğ’ x} = congruenceâ‚(ğ’) (proof{x})
    proof {âˆ}   = reflexivity(_â‰¡_)
    proof {ğ’-fixpoint i} = reflexivity(_â‰¡_)

instance
  [+]-absorberáµ£ : Absorberáµ£(_+_)(âˆ)
  Absorberáµ£.proof [+]-absorberáµ£ = reflexivity(_â‰¡_)

instance
  [+]-absorberâ‚— : Absorberâ‚—(_+_)(âˆ)
  [+]-absorberâ‚— = intro(\{x} â†’ proof{x}) where
    proof : Names.Absorberâ‚—(_+_)(âˆ)
    proof {ğŸ}   = reflexivity(_â‰¡_)
    proof {ğ’ x} = congruenceâ‚(ğ’) (proof{x}) ğŸ– ğ’-fixpoint
    proof {âˆ}   = reflexivity(_â‰¡_)
    proof {ğ’-fixpoint i} = {!!}

open import Data.Option as Option using (Option ; Some ; None)
import      Data.Option.Functions as Option

to-â„• : â„•âˆ â†’ Option(â„•)
to-â„• ğŸ     = Some â„•.ğŸ
to-â„• (ğ’ n) = Option.map â„•.ğ’(to-â„• n)
to-â„• âˆ     = None
to-â„• (ğ’-fixpoint i) = None

from-â„• : â„• â†’ â„•âˆ
from-â„• â„•.ğŸ      = ğŸ
from-â„• (â„•.ğ’(n)) = ğ’(from-â„•(n))

to-â„•-finite : (n : â„•âˆ) â†’ â¦ƒ IsTrue(isFinite n) â¦„ â†’ â„•
to-â„•-finite ğŸ     = â„•.ğŸ
to-â„•-finite (ğ’ n) = â„•.ğ’(to-â„•-finite n)

open import Type.Identity
open import Type.Identity.Proofs

open import Data.Boolean.Equiv.Path
open import Data.Option.Equiv.Path
open import Numeral.Natural.Equiv.Path

ğŸ-âˆ-inequality : (ğŸ â‰¢ âˆ)
ğŸ-âˆ-inequality = Bool-different-values âˆ˜ congruenceâ‚(not) âˆ˜ congruenceâ‚(isFinite)

ğŸ-ğ’-inequality : âˆ€{x} â†’ (ğŸ â‰¢ ğ’(x))
ğŸ-ğ’-inequality = Bool-different-values âˆ˜ congruenceâ‚(not) âˆ˜ congruenceâ‚(isZero)

instance
  from-â„•-function : Function â¦ƒ Id-equiv â¦„ â¦ƒ Path-equiv â¦„ from-â„•
  Function.congruence from-â„•-function intro = reflexivity(_â‰¡_)

instance
  to-â„•-function : Function â¦ƒ Path-equiv â¦„ â¦ƒ Id-equiv â¦„ to-â„•
  Function.congruence to-â„•-function = subâ‚‚(_â‰¡_)(Id) âˆ˜ congruenceâ‚(to-â„•)

open import Logic.Predicate
open import Logic.Propositional
open import Structure.Function.Domain
import      Structure.Function.Names as Names
open import Structure.Function.Domain.Proofs
open import Type.Size

instance
  â„•âˆ-bijection : (â„•âˆ â‰ Option(â„•)) â¦ƒ Path-equiv â¦„ â¦ƒ Id-equiv â¦„
  âˆƒ.witness â„•âˆ-bijection = to-â„•
  âˆƒ.proof â„•âˆ-bijection = {!inverse-to-bijective â¦ƒ _ â¦„ â¦ƒ _ â¦„ {f = Option.partialMap âˆ from-â„•}{fâ»Â¹ = to-â„•}!} where
    invâ‚— : Names.Inverses (Option.partialMap âˆ from-â„•) to-â„•
    invâ‚— {ğŸ}   = reflexivity(_â‰¡_)
    invâ‚— {ğ’ x} =
      (Option.partialMap âˆ from-â„• âˆ˜ to-â„•) (ğ’(x))          ğŸ–[ _â‰¡_ ]-[]
      Option.partialMap âˆ from-â„• (Option.map â„•.ğ’(to-â„• x)) ğŸ–[ _â‰¡_ ]-[ {!!} ]
      Option.partialMap âˆ (from-â„• âˆ˜ â„•.ğ’) (to-â„• x)         ğŸ–[ _â‰¡_ ]-[ {!!} ]
      Option.partialMap âˆ (ğ’ âˆ˜ from-â„•) (to-â„• x)           ğŸ–[ _â‰¡_ ]-[ {!!} ]
      ğ’(Option.partialMap âˆ from-â„• (to-â„• x))              ğŸ–[ _â‰¡_ ]-[ congruenceâ‚(ğ’) (invâ‚—{x}) ]
      ğ’(x) ğŸ–-end
    invâ‚— {âˆ}   = reflexivity(_â‰¡_)
    invâ‚— {ğ’-fixpoint i} = {!!}

    inváµ£ : Names.Inverses to-â„• (Option.partialMap âˆ from-â„•)
    inváµ£ {None}          = reflexivity(_â‰¡_)
    inváµ£ {Some â„•.ğŸ}      = reflexivity(_â‰¡_)
    inváµ£ {Some (â„•.ğ’(x))} =
      (to-â„• âˆ˜ Option.partialMap âˆ from-â„•) (Some(â„•.ğ’ x)) ğŸ–[ _â‰¡_ ]-[]
      to-â„• (from-â„• (â„•.ğ’(x)))                            ğŸ–[ _â‰¡_ ]-[]
      to-â„• (ğ’(from-â„• x))                                ğŸ–[ _â‰¡_ ]-[]
      Option.map â„•.ğ’(to-â„•(from-â„• x))                    ğŸ–[ _â‰¡_ ]-[ congruenceâ‚(Option.map â„•.ğ’) (inváµ£ {Some x}) ]
      Option.map â„•.ğ’ (Some x)                           ğŸ–[ _â‰¡_ ]-[]
      Some(â„•.ğ’ x)                                       ğŸ–-end

    instance
      inv : Inverse to-â„• (Option.partialMap âˆ from-â„•)
      inv = [âˆ§]-intro (intro invâ‚—) (intro inváµ£)
  {-injective-surjective-to-bijective â¦ƒ _ â¦„ â¦ƒ _ â¦„ (to-â„•) where
    instance
      inj : Injective â¦ƒ Path-equiv â¦„ â¦ƒ Id-equiv â¦„ (to-â„•)
      Injective.proof inj {x}{y} p = {!!}
    instance
      surj : Surjective â¦ƒ Id-equiv â¦„ (to-â„•)-}

instance
  [â‰¤]-reflexivity : Reflexivity(_â‰¤_)
  [â‰¤]-reflexivity = intro(\{x} â†’ p{x}) where
    p : Names.Reflexivity(_â‰¤_)
    p{ğŸ}   = <>
    p{ğ’ x} = p{x}
    p{âˆ}   = <>
    p{ğ’-fixpoint i} = <>

[â‰¤]áµ£-of-âˆ : âˆ€{x} â†’ (x â‰¤ âˆ)
[â‰¤]áµ£-of-âˆ {ğŸ}    = <>
[â‰¤]áµ£-of-âˆ {ğ’(x)} = <>
[â‰¤]áµ£-of-âˆ {âˆ}    = <>
[â‰¤]áµ£-of-âˆ {ğ’-fixpoint i} = <>

[â‰¤]â‚—-of-âˆ : âˆ€{x} â†’ (âˆ â‰¤ x) â†’ (x â‰¡ âˆ)
[â‰¤]â‚—-of-âˆ {âˆ}       p = reflexivity(_â‰¡_)
[â‰¤]â‚—-of-âˆ {ğ’ âˆ}     p = ğ’-fixpoint
[â‰¤]â‚—-of-âˆ {ğ’ (ğ’ x)} p = congruenceâ‚(ğ’) ([â‰¤]â‚—-of-âˆ {ğ’ x} p) ğŸ– ğ’-fixpoint
[â‰¤]â‚—-of-âˆ {ğ’(ğ’-fixpoint i)} p = {!!}
[â‰¤]â‚—-of-âˆ {ğ’-fixpoint i} p = {!ğ’-fixpoint!}

[â‰¤]-antisymmetry : Antisymmetry(_â‰¤_)(_â‰¡_)
[â‰¤]-antisymmetry = intro(\{x} â†’ p{x}) where
  p : Names.Antisymmetry(_â‰¤_)(_â‰¡_)
  p {ğŸ}   {ğŸ}   ab ba = reflexivity(_â‰¡_)
  p {ğ’ a} {ğ’ b} ab ba = congruenceâ‚(ğ’) (p{a}{b} ab ba)
  p {ğ’ a} {âˆ}   ab ba = congruenceâ‚(ğ’) (p{a}{âˆ} ([â‰¤]áµ£-of-âˆ{a}) ba) ğŸ– ğ’-fixpoint
  p {âˆ}   {ğ’ b} ab ba = {!!}
  p {âˆ}   {âˆ}   ab ba = reflexivity(_â‰¡_)
  p {ğ’ a} {ğ’-fixpoint i} ab ba = {!!}
  p {âˆ} {ğ’-fixpoint i} ab ba = {!!}
  p {ğ’-fixpoint i} {ğ’ b} ab ba = {!!}
  p {ğ’-fixpoint i} {âˆ} ab ba = {!!}
  p {ğ’-fixpoint i} {ğ’-fixpoint iâ‚} ab ba = {!!}
