module Numeral.Finite.Recursion where

open import Data
open import Logic.Propositional
import      Lvl
open import Numeral.Finite
open import Numeral.Finite.Relation.Order
open import Numeral.Finite.Relation.Order.Proofs
open import Numeral.Natural
import      Numeral.Natural.Relation as â„•
open import Type

private variable â„“ : Lvl.Level
private variable bâ‚ bâ‚‚ N : â„•
private variable n x y xâ‚ xâ‚‚ yâ‚ yâ‚‚ : ğ•Ÿ(N)

module _
  (T : âˆ€{n} â†’ ğ•Ÿ(n) â†’ Type{â„“})
  (zero : âˆ€{N} â†’ â¦ƒ pos : â„•.Positive(N) â¦„ â†’ T{N}(minimum))
  (succ : âˆ€{N} â†’ (i : ğ•Ÿ(N)) â†’ T(ğ’(i)))
  where

  ğ•Ÿ-case : âˆ€{N} â†’ (n : ğ•Ÿ(N)) â†’ T(n)
  ğ•Ÿ-case ğŸ      = zero
  ğ•Ÿ-case (ğ’(i)) = succ i

module _
  (T : âˆ€{n} â†’ ğ•Ÿ(n) â†’ Type{â„“})
  (base : âˆ€{N} â†’ â¦ƒ pos : â„•.Positive(N) â¦„ â†’ T{N}(minimum))
  (step : âˆ€{N} â†’ (i : ğ•Ÿ(N)) â†’ T(i) â†’ T(ğ’(i)))
  where

  ğ•Ÿ-elim : âˆ€{N} â†’ (n : ğ•Ÿ(N)) â†’ T(n)
  ğ•Ÿ-elim{ğ’ N} ğŸ     = base
  ğ•Ÿ-elim{ğ’ N} (ğ’ n) = step n (ğ•Ÿ-elim{N} n)

module _
  (P : âˆ€{N} â†’ ğ•Ÿ(N) â†’ Type{â„“})
  (rec : âˆ€{N} â†’ (n : ğ•Ÿ(N)) â†’ (âˆ€{I} â†’ (i : ğ•Ÿ(I)) â†’ (i < n) â†’ P(i)) â†’ P(n))
  where

  ğ•Ÿ-strong-recursion : âˆ€{N} â†’ (n : ğ•Ÿ(N)) â†’ P(n)
  ğ•Ÿ-strong-recursion n = ğ•Ÿ-elim(\n â†’ âˆ€{I} â†’ (i : ğ•Ÿ(I)) â†’ (i < n) â†’ P(i))
    (\i imin â†’ empty([<]-minimumáµ£ {a = i} imin))
    (\n prev i iğ’n â†’ rec i (\j ji â†’ prev j ([<][â‰¤]-subtransitivityáµ£-raw {a = j}{b = i}{c = n} ji ([â†”]-to-[â†] ([â‰¤][<]-convert {a = i}{b = n}) iğ’n))))
    (ğ’(n)) n ([<]-of-successor {a = n})

open import Functional

-- TODO: Is this necessary?
ğ•Ÿ-strong-recursionâ‚‚ : (P : âˆ€{Nâ‚ Nâ‚‚} â†’ ğ•Ÿ(Nâ‚) â†’ ğ•Ÿ(Nâ‚‚) â†’ Type{â„“}) â†’ (âˆ€{X Y} â†’ (x : ğ•Ÿ(X)) â†’ (y : ğ•Ÿ(Y)) â†’ (âˆ€{I J} â†’ (i : ğ•Ÿ(I)) â†’ (j : ğ•Ÿ(J)) â†’ (i < x) âˆ¨ ((i â‰¤ x) âˆ§ (j < y)) â†’ P i j) â†’ P x y) â†’ (âˆ€{Nâ‚ Nâ‚‚} â†’ (x : ğ•Ÿ(Nâ‚)) â†’ (y : ğ•Ÿ(Nâ‚‚)) â†’ P x y)
ğ•Ÿ-strong-recursionâ‚‚ P rec x y =
  ğ•Ÿ-strong-recursion(\x â†’ âˆ€{Y} â†’ (y : ğ•Ÿ(Y)) â†’ P x y) (\x prevX y â†’
  ğ•Ÿ-strong-recursion(\y â†’ âˆ€{X} â†’ (xâ‚‚ : ğ•Ÿ(X)) â†’ (xâ‚‚ â‰¤ x) â†’ P xâ‚‚ y) (\y prevY x xâ‚‚x â†’ rec x y \i j â†’ [âˆ¨]-elim
    (\ix â†’ prevX i ([<][â‰¤]-subtransitivityáµ£-raw {a = i}{b = x} ix xâ‚‚x) j)
    (\([âˆ§]-intro ix jy) â†’ prevY j jy i ([â‰¤]-transitivity-raw {a = i}{b = x} ix xâ‚‚x))
  ) y x ([â‰¤]-reflexivity-raw {a = x}))
  x y
