module Numeral.Natural.Relation.Order.Existence.Proofs{â„“} where

import Lvl
open import Data.Tuple as Tuple using (_â¨¯_ ; _,_)
open import Functional
open import Logic.Propositional{â„“}
open import Logic.Propositional.Theorems{â„“}
open import Logic.Predicate{â„“}{Lvl.ğŸ}
open import Numeral.Natural
open import Numeral.Natural.Oper
open import Numeral.Natural.Oper.Properties{â„“}
open import Numeral.Natural.Induction{â„“}
import      Numeral.Natural.Relation.Order{â„“} as [â‰¤def]
open import Numeral.Natural.Relation.Order.Existence{â„“}
open import Relator.Equals{â„“}{Lvl.ğŸ}
open import Relator.Equals.Proofs{â„“}{Lvl.ğŸ}
open import Structure.Operator.Properties{â„“}{Lvl.ğŸ}
open import Structure.Relator.Ordering{â„“}{Lvl.ğŸ}
open import Structure.Relator.Properties{â„“}{Lvl.ğŸ}
open import Type

[â‰¡]-to-[â‰¤] : âˆ€{x y : â„•} â†’ (x â‰¡ y) â†’ (x â‰¤ y)
[â‰¡]-to-[â‰¤] xâ‰¡y = [âˆƒ]-intro 0 â¦ƒ xâ‰¡y â¦„

[â‰¤]-minimum : âˆ€{x : â„•} â†’ (0 â‰¤ x)
[â‰¤]-minimum {x} = [âˆƒ]-intro x â¦ƒ [+]-identityâ‚— â¦„
-- [âˆƒ]-intro {â„•} {\n â†’ 0 + n â‰¡ x} (x) â¦ƒ [+]-identityâ‚— â¦„

[â‰¤][0]áµ£ : âˆ€{x : â„•} â†’ (x â‰¤ 0) â†” (x â‰¡ 0)
[â‰¤][0]áµ£ {ğŸ} = [â†”]-intro l r where
  l : (ğŸ â‰¤ 0) â† (ğŸ â‰¡ 0)
  l refl = [â‰¡]-to-[â‰¤] refl

  r : (ğŸ â‰¤ 0) â†’ (ğŸ â‰¡ 0)
  r _ = [â‰¡]-intro
[â‰¤][0]áµ£ {ğ’(n)} = [â†”]-intro l r where
  l : (ğ’(n) â‰¤ 0) â† (ğ’(n) â‰¡ 0)
  l ()

  r : (ğ’(n) â‰¤ 0) â†’ (ğ’(n) â‰¡ 0)
  r ([âˆƒ]-intro _ â¦ƒ â¦„ )

[â‰¤][0]áµ£-negation : âˆ€{x : â„•} â†’ Â¬(ğ’(x) â‰¤ 0)
[â‰¤][0]áµ£-negation {x} (Sxâ‰¤0) = [ğ’]-not-0([â†”]-elimáµ£([â‰¤][0]áµ£ {ğ’(x)}) (Sxâ‰¤0))

[â‰¤]-successor : âˆ€{a b : â„•} â†’ (a â‰¤ b) â†’ (a â‰¤ ğ’(b))
[â‰¤]-successor ([âˆƒ]-intro(n) â¦ƒ proof â¦„) = [âˆƒ]-intro (ğ’(n)) â¦ƒ [â‰¡]-with(ğ’) (proof) â¦„
-- a + n â‰¡ b //f
-- a + ? â‰¡ ğ’(b) //What value works if f?
-- a + ğ’(n) â‰¡ ğ’(b)
-- ğ’(a + n) â‰¡ ğ’(b) //[â‰¡]-with(ğ’) f

[â‰¤]-predecessor : âˆ€{a b : â„•} â†’ (ğ’(a) â‰¤ b) â†’ (a â‰¤ b)
[â‰¤]-predecessor ([âˆƒ]-intro(n) â¦ƒ proof â¦„) = [âˆƒ]-intro (ğ’(n)) â¦ƒ proof â¦„

[â‰¤]-with-[ğ’] : âˆ€{a b : â„•} â†’ (a â‰¤ b) â†’ (ğ’(a) â‰¤ ğ’(b))
[â‰¤]-with-[ğ’] {a} {b} ([âˆƒ]-intro n â¦ƒ f â¦„) =
  [âˆƒ]-intro
    (n)
   â¦ƒ
      ([+1]-commutativity {a} {n}) -- ğ’(a)+n = a+ğ’(n)
      ğŸ– ([â‰¡]-with(ğ’) f) -- ğ’(a+n)=a+ğ’(n) = ğ’(b)
    â¦„

[â‰¤]-without-[ğ’] : âˆ€{a b : â„•} â†’ (a â‰¤ b) â† (ğ’(a) â‰¤ ğ’(b))
[â‰¤]-without-[ğ’] {ğŸ}   {b}    (_)                    = [â‰¤]-minimum
[â‰¤]-without-[ğ’] {ğ’(a)}{ğŸ}    ()
[â‰¤]-without-[ğ’] {ğ’(a)}{ğ’(b)} ([âˆƒ]-intro(n) â¦ƒ proof â¦„) = [â‰¤]-with-[ğ’] {a}{b} ([â‰¤]-without-[ğ’] {a}{b} ([âˆƒ]-intro(n) â¦ƒ [ğ’]-injectivity proof â¦„))

[â‰¤][ğ’]â‚— : âˆ€{x : â„•} â†’ Â¬(ğ’(x) â‰¤ x)
[â‰¤][ğ’]â‚— {ğŸ}    (1â‰¤0)    = [â‰¤][0]áµ£-negation{0}(1â‰¤0)
[â‰¤][ğ’]â‚— {ğ’(n)} (SSnâ‰¤Sn) = [â‰¤][ğ’]â‚— {n} ([â‰¤]-without-[ğ’] {ğ’(n)}{n} (SSnâ‰¤Sn))

instance
  [â‰¤]-transitivity : Transitivity (_â‰¤_)
  transitivity â¦ƒ [â‰¤]-transitivity â¦„ {a}{b}{c} ([âˆƒ]-intro nâ‚ â¦ƒ a+nâ‚â‰¡b â¦„) ([âˆƒ]-intro nâ‚‚ â¦ƒ b+nâ‚‚â‰¡c â¦„) =
    [âˆƒ]-intro
      (nâ‚ + nâ‚‚)
     â¦ƒ
        (symmetry ([+]-associativity {a} {nâ‚} {nâ‚‚})) -- a+(nâ‚+nâ‚‚) = (a+nâ‚)+nâ‚‚
        ğŸ– ([â‰¡]-with(expr â†¦ expr + nâ‚‚) (a+nâ‚â‰¡b)) -- (a+nâ‚)+nâ‚‚ = b+nâ‚‚
        ğŸ– (b+nâ‚‚â‰¡c) -- b+nâ‚‚ = c
      â¦„ -- a+(nâ‚+nâ‚‚) = c

instance
  [â‰¤]-reflexivity : Reflexivity (_â‰¤_)
  reflexivity â¦ƒ [â‰¤]-reflexivity â¦„ = [â‰¡]-to-[â‰¤] [â‰¡]-intro

instance
  [â‰¤]-antisymmetry : Antisymmetry (_â‰¤_) (_â‰¡_)
  antisymmetry â¦ƒ [â‰¤]-antisymmetry â¦„ {a} {b} ([âˆƒ]-intro(nâ‚) â¦ƒ a+nâ‚â‰¡b â¦„) ([âˆƒ]-intro(nâ‚‚) â¦ƒ b+nâ‚‚â‰¡a â¦„) = [â‰¡]-elimáµ£ (nâ‚â‰¡0) {n â†¦ (a + n â‰¡ b)} (a+nâ‚â‰¡b) where
    nâ‚+nâ‚‚â‰¡0 : ((nâ‚ + nâ‚‚) â‰¡ 0)
    nâ‚+nâ‚‚â‰¡0 =
      [+]-injectivityáµ£(
        (symmetry([+]-associativity {a} {nâ‚} {nâ‚‚}))
        ğŸ– ([â‰¡]-with(expr â†¦ expr + nâ‚‚) a+nâ‚â‰¡b)
        ğŸ– b+nâ‚‚â‰¡a
      )
    nâ‚â‰¡0 : (nâ‚ â‰¡ 0)
    nâ‚â‰¡0 = [+]-sum-is-0â‚— {nâ‚} {nâ‚‚} nâ‚+nâ‚‚â‰¡0
  -- a+nâ‚ = b
  -- (a+nâ‚)+nâ‚‚ = b+nâ‚‚
  -- (a+nâ‚)+nâ‚‚ = a
  -- a+(nâ‚+nâ‚‚) = a
  -- a+(nâ‚+nâ‚‚) = a+0
  -- nâ‚+nâ‚‚ = 0
  -- a = b

instance
  [â‰¤]-weakPartialOrder : Weak.PartialOrder (_â‰¤_) (_â‰¡_)
  [â‰¤]-weakPartialOrder = record{
      antisymmetry = [â‰¤]-antisymmetry;
      transitivity = [â‰¤]-transitivity;
      reflexivity  = [â‰¤]-reflexivity
    }

[<]-minimum : âˆ€{x : â„•} â†’ (0 < ğ’(x))
[<]-minimum {x} = [â‰¤]-with-[ğ’] {0} ([â‰¤]-minimum)

[â‰¥]-is-[â‰®] : âˆ€{a b : â„•} â†’ Â¬(a < b) â† (a â‰¥ b)
[â‰¥]-is-[â‰®] {a}{b} (bâ‰¤a) (Saâ‰¤b) = [â‰¤][ğ’]â‚— (transitivity {_}{_}{ğ’(a)}{b}{a} (Saâ‰¤b) (bâ‰¤a))

-- [â‰¤]-is-[â‰¯] : âˆ€{a b : â„•} â†’ Â¬(a > b) â† (a â‰¤ b)
-- [â‰¤]-is-[â‰¯] {a}{b} = [â‰¥]-is-[â‰®] {b}{a}

-- [>]-is-[â‰°] : âˆ€{a b : â„•} â†’ Â¬(a â‰¤ b) â† (a > b)
-- [>]-is-[â‰°] {a}{b} (Sbâ‰¤a) (aâ‰¤b) = [â‰¤]-is-[â‰¯] {a}{b} (aâ‰¤b) (Sbâ‰¤a)

-- [<]-is-[â‰±] : âˆ€{a b : â„•} â†’ Â¬(a â‰¥ b) â† (a < b)
-- [<]-is-[â‰±] {a}{b} = [>]-is-[â‰°] {b}{a}

instance
  [â‰¤]-totality : SymmetricallyTotal(_â‰¤_)
  converseTotal â¦ƒ [â‰¤]-totality â¦„ {ğŸ}   {ğŸ}    = [âˆ¨]-introâ‚— ([â‰¡]-to-[â‰¤] [â‰¡]-intro)
  converseTotal â¦ƒ [â‰¤]-totality â¦„ {ğ’(a)}{ğŸ}    = [âˆ¨]-introáµ£ ([â‰¤]-minimum)
  converseTotal â¦ƒ [â‰¤]-totality â¦„ {ğŸ}   {ğ’(b)} = [âˆ¨]-introâ‚— ([â‰¤]-minimum)
  converseTotal â¦ƒ [â‰¤]-totality â¦„ {ğ’(a)}{ğ’(b)} = [âˆ¨]-elim ([âˆ¨]-introâ‚— âˆ˜ ([â‰¤]-with-[ğ’] {a}{b})) ([âˆ¨]-introáµ£ âˆ˜ ([â‰¤]-with-[ğ’] {b}{a})) (converseTotal â¦ƒ [â‰¤]-totality â¦„ {a}{b})

[â‰¤]-equivalence : âˆ€{x y} â†’ (x â‰¤ y) â†” (x [â‰¤def].â‰¤ y)
[â‰¤]-equivalence{x}{y} = [â†”]-intro (l{x}{y}) (r{x}{y}) where
  l : âˆ€{x y} â†’ (x â‰¤ y) â† (x [â‰¤def].â‰¤ y)
  l{ğŸ}   {y}    ([â‰¤def].[â‰¤]-minimum)      = [âˆƒ]-intro(y) â¦ƒ [â‰¡]-intro â¦„
  l{ğ’(x)}{ğŸ}    ()
  l{ğ’(x)}{ğ’(y)} ([â‰¤def].[â‰¤]-with-[ğ’] â¦ƒ proof â¦„) = [â‰¤]-with-[ğ’] {x}{y} (l{x}{y} (proof))

  r : âˆ€{x y} â†’ (x â‰¤ y) â†’ (x [â‰¤def].â‰¤ y)
  r{ğŸ}   {y}    ([âˆƒ]-intro(z) â¦ƒ ğŸ+zâ‰¡y   â¦„) = [â‰¤def].[â‰¤]-minimum
  r{ğ’(x)}{ğŸ}    ([âˆƒ]-intro(z) â¦ƒ â¦„)
  r{ğ’(x)}{ğ’(y)} ([âˆƒ]-intro(z) â¦ƒ ğ’x+zâ‰¡ğ’y â¦„) = [â‰¤def].[â‰¤]-with-[ğ’] â¦ƒ r{x}{y} ([âˆƒ]-intro(z) â¦ƒ [ğ’]-injectivity(ğ’x+zâ‰¡ğ’y) â¦„ ) â¦„
