module Numeral.Natural.Relation where

import Level as Lvl
open import Logic
open import Numeral.Natural
open import Numeral.Natural.Oper
open import Relator.Equals Lvl.ğŸ

[â„•]-induction : {X : â„• â†’ Set} â†’ X(ğŸ) â†’ ((i : â„•) â†’ X(i) â†’ X(ğ’(i))) â†’ (n : â„•) â†’ X(n)
[â„•]-induction base next ğŸ = base
[â„•]-induction base next (ğ’(n)) = next(n)([â„•]-induction base next n)

[+]-identityâ‚— : âˆ€ {x : â„•} â†’ (0 + x) â‰¡ x
[+]-identityâ‚— {x} = [â„•]-induction base next x where
  base : ((0 + 0) â‰¡ 0)
  base = [â‰¡]-intro

  next : âˆ€ (i : â„•) â†’ ((0 + i) â‰¡ i) â†’ ((0 + ğ’(i)) â‰¡ ğ’(i))
  next _ = [â‰¡]-with-[ ğ’ ]

[+]-identityáµ£ : âˆ€ {x : â„•} â†’ (x + 0) â‰¡ x
[+]-identityáµ£ {x} = [â„•]-induction base next x where
  base : ((0 + 0) â‰¡ 0)
  base = [â‰¡]-intro

  next : âˆ€ (i : â„•) â†’ ((i + 0) â‰¡ i) â†’ ((ğ’(i) + 0) â‰¡ ğ’(i))
  next _ = [â‰¡]-with-[ ğ’ ]

[+]-associativity : âˆ€ {x y z : â„•} â†’ ((x + y) + z) â‰¡ (x + (y + z))
[+]-associativity {x} {y} {z} = [â„•]-induction (base x y) (next x y) z where
  base : âˆ€ (x y : â„•) â†’ ((x + y) + 0) â‰¡ (x + (y + 0))
  base _ _ = [â‰¡]-intro

  next : âˆ€ (x y : â„•) â†’ (i : â„•) â†’ ((x + y) + i) â‰¡ (x + (y + i)) â†’ ((x + y) + ğ’(i)) â‰¡ (x + (y + ğ’(i)))
  next _ _ _ = [â‰¡]-with-[ ğ’ ]

[+1]-commutativity : âˆ€ {x y : â„•} â†’ (ğ’(x) + y) â‰¡ (x + ğ’(y))
[+1]-commutativity {x} {y} = [â„•]-induction (base x) (next x) y where
  base : âˆ€ (x : â„•) â†’ (ğ’(x) + 0) â‰¡ (x + ğ’(0))
  base _ = [â‰¡]-intro

  next : âˆ€ (x : â„•) â†’ (i : â„•) â†’ (ğ’(x) + i) â‰¡ (x + ğ’(i)) â†’ (ğ’(x) + ğ’(i)) â‰¡ (x + ğ’(ğ’(i)))
  next x i = [â‰¡]-with-[ ğ’ ]

[+]-commutativity : âˆ€ {x y : â„•} â†’ (x + y) â‰¡ (y + x)
[+]-commutativity {x} {y} = [â„•]-induction (base x) (next x) y where
  base : âˆ€ (x : â„•) â†’ (x + 0) â‰¡ (0 + x)
  base _ = [â‰¡]-symmetry([â‰¡]-transitivity([âˆ§]-intro [+]-identityâ‚— ([â‰¡]-symmetry [+]-identityáµ£)))
  -- (âˆ€x. 0+x = x) âˆ§ (âˆ€x. x = x+0) // [âˆ§]-intro [1] [2]
  --   âˆ€x. 0+x = x //[+]-identityâ‚— [1]

  --   âˆ€x. x+0 = x //[+]-identityáµ£
  --   âˆ€x. x = x+0 //[â‰¡]-symmetry(..) [2]
  -- (âˆ€x. 0+x = x+0) // [â‰¡]-transitivity(..)

  next : âˆ€ (x i : â„•) â†’ (x + i) â‰¡ (i + x) â†’ (x + ğ’(i)) â‰¡ (ğ’(i) + x)
  next x i eq =
    [â‰¡]-transitivity([âˆ§]-intro
      ([â‰¡]-with-[ ğ’ ]
        eq
      )

      ([â‰¡]-symmetry(
        [+1]-commutativity {i} {x}
      ))
    )
  --   âˆ€xâˆ€i. x+i = i+x //eq
  --   âˆ€xâˆ€i. ğ’(x+i) = ğ’(i+x) //[â‰¡]-with-[ ğ’ ](..)
  --   âˆ€xâˆ€i. x+ğ’(i) = i+ğ’(x) //x + ğ’(y) = ğ’(x + y) (Definition of _+_) [1]

  --   âˆ€xâˆ€i. ğ’(i)+x = i+ğ’(x) //[+1]-commutativity
  --   âˆ€xâˆ€i. i+ğ’(x) = ğ’(i)+x //[â‰¡]-symmetry [2]
  -- âˆ€xâˆ€i. x+ğ’(i) = ğ’(i)+x //[â‰¡]-transitivity [1] [2]

[â‹…]-absorberâ‚— : âˆ€ {x} â†’ (0 â‹… x) â‰¡ 0
[â‹…]-absorberâ‚— {x} = [â„•]-induction base next x where
  base : (0 â‹… 0) â‰¡ 0
  base = [â‰¡]-reflexivity

  next : âˆ€ (x : â„•) â†’ (0 â‹… x) â‰¡ 0 â†’ (0 â‹… ğ’(x)) â‰¡ 0
  next _ eq = [â‰¡]-with-[(Î» x â†’ 0 + x)] eq

[â‹…]-absorberáµ£ : âˆ€ {x : â„•} â†’ (x â‹… 0) â‰¡ 0
[â‹…]-absorberáµ£ = [â‰¡]-intro

[â‹…]-identityâ‚— : âˆ€ {x : â„•} â†’ (1 â‹… x) â‰¡ x
[â‹…]-identityâ‚— {x} = [â„•]-induction base next x where
  base : ((1 â‹… 0) â‰¡ 0)
  base = [â‰¡]-reflexivity

  next : (i : â„•) â†’ ((1 â‹… i) â‰¡ i) â†’ ((1 â‹… ğ’(i)) â‰¡ ğ’(i))
  next i eq =
    [â‰¡]-transitivity([âˆ§]-intro
      ([+]-commutativity {1} {1 â‹… i})
      ([â‰¡]-with-[ ğ’ ] eq)
    )
--   1 + 1â‹…i = 1â‹…i + 1 //[+]-commutativity

--   1â‹…i = i //eq
--   ğ’(1â‹…i) = ğ’(i) //[â‰¡]-with[ ğ’ ] (..)
--   1â‹…i + 1 = ğ’(i) //Definition: (+)
-- 1 + 1â‹…i = ğ’(i)
-- 1 â‹… ğ’(i) = ğ’(i) //1 â‹… ğ’(y) = 1 + (1 â‹… y) (Definition: (â‹…))

[â‹…]-identityáµ£ : âˆ€ {x : â„•} â†’ (x â‹… 1) â‰¡ x
[â‹…]-identityáµ£ = [â‰¡]-intro

-- [â‹…][+]-distributivityáµ£ : âˆ€ {x y z : â„•} â†’ ((x + y) â‹… z) â‰¡ ((x â‹… z) + (y â‹… z))
-- [â‹…][+]-distributivityáµ£ {x} {y} {z} = [â„•]-induction (base x y) (next x y) z where
--   base : âˆ€ (x y : â„•) â†’ ((x + y) â‹… 0) â‰¡ ((x â‹… 0) + (y â‹… 0))
--   base _ _ = [â‰¡]-intro

--   next : âˆ€ (x y z : â„•) â†’ ((x + y) â‹… z) â‰¡ ((x â‹… z) + (y â‹… z)) â†’ ((x + y) â‹… ğ’(z)) â‰¡ ((x â‹… ğ’(z)) + (y â‹… ğ’(z)))
--   next x y z eq = eq
--     -- ((x + y) â‹… z) â‰¡ ((x â‹… z) + (y â‹… z))
--     -- (x + y) + ((x + y) â‹… z) = (x + y) + ((x â‹… z) + (y â‹… z)) //[â‰¡]-with-[(expr â†¦ (x+y) + expr)]
--     -- (x + y) â‹… ğ’(z) = (x + y) + ((x â‹… z) + (y â‹… z)) // (x + y) â‹… ğ’(z) = (x + y) + ((x + y) â‹… z) (Definition: (â‹…))

--     -- (x + y) + ((x â‹… z) + (y â‹… z)) = (x + y) + ((x â‹… z) + (y â‹… z)) //[â‰¡]-intro
--     -- = x + (y + ((x â‹… z) + (y â‹… z))) //[+]-associativity
--     -- = x + ((y + (x â‹… z)) + (y â‹… z)) //[+]-associativity
--     -- = x + (((x â‹… z) + y) + (y â‹… z)) //[+]-commutativity
--     -- = x + ((x â‹… z) + (y + (y â‹… z))) //[+]-associativity
--     -- = (x + (x â‹… z)) + (y + (y â‹… z)) //[+]-associativity
--     -- = (x â‹… ğ’(z)) + (y â‹… ğ’(z)) //Definition: (â‹…)

-- [â‹…]-associativity : âˆ€ {x y z : â„•} â†’ ((x â‹… y) â‹… z) â‰¡ (x â‹… (y â‹… z))

-- [â‹…][+]-distributivity : âˆ€ {x y z : â„•} â†’ (x â‹… (y + z)) â‰¡ (x â‹… y) + (x â‹… z)



-- Divisibility
data Even : â„• â†’ Set where
  Even0 : Even ğŸ
  Evenğ’ : {x : â„•} â†’ (Even x) â†’ (Even(ğ’(ğ’(x))))

data Odd : â„• â†’ Set where
  Odd0 : Odd (ğ’(ğŸ))
  Oddğ’ : {x : â„•} â†’ (Odd x) â†’ (Odd(ğ’(ğ’(x))))

data _divides_ : â„• â†’ â„• â†’ Set where
  Div0 : {x : â„•} â†’ x divides ğŸ
  Divğ’ : {x : â„•} â†’ {y : â„•} â†’ (x divides y) â†’ (x divides (x + y))

data _divides_withRemainder_ : â„• â†’ â„• â†’ â„• â†’ Set where
  DivRem0 : {x : â„•} â†’{r : â„•} â†’ x divides r withRemainder r
  DivRemğ’ : {x : â„•} â†’ {y : â„•} â†’ {r : â„•} â†’ (x divides y withRemainder r) â†’ (x divides (x + y) withRemainder r)

-- testAssociativityOfSuccessor1 : âˆ€ {x y} â†’ ((x + 1) + y) â‰¡ (x + (1 + y))
-- testAssociativityOfSuccessor1 {x} {y} = [+]-associativity {x} {1} {y}

-- testAssociativityOfSuccessor2 : âˆ€ {x y} â†’ (ğ’(x) + y) â‰¡ (x + (1 + y))
-- testAssociativityOfSuccessor2 {x} {y} = [+]-associativity {x} {1} {y}
